Ethereum/Theory/OpcodeLemmas.lean
@@ -71,7 +71,7 @@ theorem step_stop : ∀ (s : State),
       if s.machineState.stack.length - 0 + 0 > 1024 then .error .StackOverflow
       else
       .ok ({s with
-              machineState.gasAvailable := s.machineState.gasAvailable.natSub GasConstants.Gzero
+              machineState.gasAvailable := s.machineState.gasAvailable.subNat GasConstants.Gzero
               machineState.execLength := s.machineState.execLength + 1
               machineState.returnData := .empty
             }, .some (.success, .empty))
@@ -85,7 +85,7 @@ theorem step_stop : ∀ (s : State),
       simp [GasConstants.Gzero]
     have hgas' :
         ¬ s.machineState.gasAvailable.toNat < GasConstants.Gzero := by
-      simpa [Sat256.natSub_zero, UInt256_subzero'] using hgas
+      simpa [Sat256.subNat_zero, UInt256_subzero'] using hgas
     rw [if_neg hgas']
     simp [α, Operation.isCreate]
     by_cases hoverflow : 1024 < s.machineState.stack.length
@@ -95,7 +95,6 @@ theorem step_stop : ∀ (s : State),
       simp [bind, Except.bind]
       unfold step
       simp [MachineState.setReturnData, GasConstants.Gzero]
-      rw [Sat256.natSub_zero]
 
 theorem step_add : ∀ (s : State),
   let I_b := s.executionEnv.code
@@ -110,7 +109,7 @@ theorem step_add : ∀ (s : State),
         else
         .ok ({s with
                   machineState.stack := (a + b) :: t,
-                  machineState.gasAvailable := s.machineState.gasAvailable.natSub GasConstants.Gverylow
+                  machineState.gasAvailable := s.machineState.gasAvailable.subNat GasConstants.Gverylow
                   machineState.pc := s.machineState.pc + ⟨1⟩
                   machineState.execLength := s.machineState.execLength + 1
                   }
@@ -139,7 +138,7 @@ theorem step_add : ∀ (s : State),
         ·
           simp [hoverflow]
           have hgas0 : ¬ s.machineState.gasAvailable.toNat < GasConstants.Gverylow := by
-            simpa [Sat256.natSub_zero, UInt256_subzero'] using hgas
+            simpa [Sat256.subNat_zero, UInt256_subzero'] using hgas
           simp [bind, Except.bind]
 
           unfold step
@@ -149,8 +148,6 @@ theorem step_add : ∀ (s : State),
           apply And.intro
           · simp [UInt256_ofNat_1]
           · simp [Stack.push]; constructor
-            · simp [UInt256.add]; rfl
-            · rw [Sat256.natSub_zero]
 
 theorem step_mul : ∀ (s : State),
   let I_b := s.executionEnv.code
@@ -164,7 +161,7 @@ theorem step_mul : ∀ (s : State),
         else
         .ok ({s with
                   machineState.stack := UInt256.mul a b :: t,
-                  machineState.gasAvailable := s.machineState.gasAvailable.natSub $ GasConstants.Glow
+                  machineState.gasAvailable := s.machineState.gasAvailable.subNat $ GasConstants.Glow
                   machineState.pc := s.machineState.pc + ⟨1⟩
                   machineState.execLength := s.machineState.execLength + 1
                   }
@@ -205,7 +202,6 @@ theorem step_mul : ∀ (s : State),
           apply And.intro
           · simp [UInt256_ofNat_1]
           · simp [Stack.push, flip]
-            rw [Sat256.natSub_zero]
 
 theorem step_exp : ∀ (s : State),
   let I_b := s.executionEnv.code
@@ -222,7 +218,7 @@ theorem step_exp : ∀ (s : State),
         else
         .ok ({s with
                   machineState.stack := UInt256.exp a b :: t,
-                  machineState.gasAvailable := s.machineState.gasAvailable.natSub gasCost
+                  machineState.gasAvailable := s.machineState.gasAvailable.subNat gasCost
                   machineState.pc := s.machineState.pc + ⟨1⟩
                   machineState.execLength := s.machineState.execLength + 1
                   }
@@ -256,7 +252,6 @@ theorem step_exp : ∀ (s : State),
           apply And.intro
           · simp [UInt256_ofNat_1]
           · simp [Stack.push, flip]
-            rw [Sat256.natSub_zero]
 
 theorem step_addmod : ∀ (s : State),
   let I_b := s.executionEnv.code
@@ -270,7 +265,7 @@ theorem step_addmod : ∀ (s : State),
         else
         .ok ({s with
                   machineState.stack := UInt256.addMod a b c :: t,
-                  machineState.gasAvailable := s.machineState.gasAvailable.natSub GasConstants.Gmid
+                  machineState.gasAvailable := s.machineState.gasAvailable.subNat GasConstants.Gmid
                   machineState.pc := s.machineState.pc + ⟨1⟩
                   machineState.execLength := s.machineState.execLength + 1
                   }
@@ -309,7 +304,6 @@ theorem step_addmod : ∀ (s : State),
           apply And.intro
           · simp [UInt256_ofNat_1]
           · simp [Stack.push, Ethereum.State.calldataload]
-            rw [Sat256.natSub_zero]
 
 theorem step_mulmod : ∀ (s : State),
   let I_b := s.executionEnv.code
@@ -323,7 +317,7 @@ theorem step_mulmod : ∀ (s : State),
         else
         .ok ({s with
                   machineState.stack := UInt256.mulMod a b c :: t,
-                  machineState.gasAvailable := s.machineState.gasAvailable.natSub GasConstants.Gmid
+                  machineState.gasAvailable := s.machineState.gasAvailable.subNat GasConstants.Gmid
                   machineState.pc := s.machineState.pc + ⟨1⟩
                   machineState.execLength := s.machineState.execLength + 1
                   }
@@ -362,7 +356,6 @@ theorem step_mulmod : ∀ (s : State),
           apply And.intro
           · simp [UInt256_ofNat_1]
           · simp [Stack.push, Ethereum.State.blockHash]
-            rw [Sat256.natSub_zero]
 
 theorem step_sdiv : ∀ (s : State),
   let I_b := s.executionEnv.code
@@ -376,7 +369,7 @@ theorem step_sdiv : ∀ (s : State),
         else
         .ok ({s with
                   machineState.stack := UInt256.sdiv a b :: t,
-                  machineState.gasAvailable := s.machineState.gasAvailable.natSub GasConstants.Glow
+                  machineState.gasAvailable := s.machineState.gasAvailable.subNat GasConstants.Glow
                   machineState.pc := s.machineState.pc + ⟨1⟩
                   machineState.execLength := s.machineState.execLength + 1
                   }
@@ -414,7 +407,6 @@ theorem step_sdiv : ∀ (s : State),
           apply And.intro
           · simp [UInt256_ofNat_1]
           · simp [Stack.push, blobhash]
-            rw [Sat256.natSub_zero]
 
 theorem step_mod : ∀ (s : State),
   let I_b := s.executionEnv.code
@@ -428,7 +420,7 @@ theorem step_mod : ∀ (s : State),
         else
         .ok ({s with
                   machineState.stack := UInt256.mod a b :: t,
-                  machineState.gasAvailable := s.machineState.gasAvailable.natSub GasConstants.Glow
+                  machineState.gasAvailable := s.machineState.gasAvailable.subNat GasConstants.Glow
                   machineState.pc := s.machineState.pc + ⟨1⟩
                   machineState.execLength := s.machineState.execLength + 1
                   }
@@ -466,7 +458,6 @@ theorem step_mod : ∀ (s : State),
           apply And.intro
           · simp [UInt256_ofNat_1]
           · simp [Stack.push]
-            rw [Sat256.natSub_zero]
 
 theorem step_smod : ∀ (s : State),
   let I_b := s.executionEnv.code
@@ -480,7 +471,7 @@ theorem step_smod : ∀ (s : State),
         else
         .ok ({s with
                   machineState.stack := UInt256.smod a b :: t,
-                  machineState.gasAvailable := s.machineState.gasAvailable.natSub GasConstants.Glow
+                  machineState.gasAvailable := s.machineState.gasAvailable.subNat GasConstants.Glow
                   machineState.pc := s.machineState.pc + ⟨1⟩
                   machineState.execLength := s.machineState.execLength + 1
                   }
@@ -518,7 +509,6 @@ theorem step_smod : ∀ (s : State),
           apply And.intro
           · simp [UInt256_ofNat_1]
           · simp [Stack.push]
-            rw [Sat256.natSub_zero]
 
 theorem step_signextend : ∀ (s : State),
   let I_b := s.executionEnv.code
@@ -532,7 +522,7 @@ theorem step_signextend : ∀ (s : State),
         else
         .ok ({s with
                   machineState.stack := UInt256.signextend a b :: t,
-                  machineState.gasAvailable := s.machineState.gasAvailable.natSub GasConstants.Glow
+                  machineState.gasAvailable := s.machineState.gasAvailable.subNat GasConstants.Glow
                   machineState.pc := s.machineState.pc + ⟨1⟩
                   machineState.execLength := s.machineState.execLength + 1
                   }
@@ -570,7 +560,6 @@ theorem step_signextend : ∀ (s : State),
           apply And.intro
           · simp [UInt256_ofNat_1]
           · simp [Stack.push]
-            rw [Sat256.natSub_zero]
 
 theorem step_sub : ∀ (s : State),
   let I_b := s.executionEnv.code
@@ -584,7 +573,7 @@ theorem step_sub : ∀ (s : State),
         else
         .ok ({s with
                   machineState.stack := UInt256.sub a b :: t,
-                  machineState.gasAvailable := s.machineState.gasAvailable.natSub GasConstants.Gverylow
+                  machineState.gasAvailable := s.machineState.gasAvailable.subNat GasConstants.Gverylow
                   machineState.pc := s.machineState.pc + ⟨1⟩
                   machineState.execLength := s.machineState.execLength + 1
                   }
@@ -625,7 +614,6 @@ theorem step_sub : ∀ (s : State),
           apply And.intro
           · simp [UInt256_ofNat_1]
           · simp [Stack.push]
-            rw [Sat256.natSub_zero]
 
 theorem step_div : ∀ (s : State),
   let I_b := s.executionEnv.code
@@ -639,7 +627,7 @@ theorem step_div : ∀ (s : State),
         else
         .ok ({s with
                   machineState.stack := UInt256.div a b :: t,
-                  machineState.gasAvailable := s.machineState.gasAvailable.natSub GasConstants.Glow
+                  machineState.gasAvailable := s.machineState.gasAvailable.subNat GasConstants.Glow
                   machineState.pc := s.machineState.pc + ⟨1⟩
                   machineState.execLength := s.machineState.execLength + 1
                   }
@@ -680,7 +668,6 @@ theorem step_div : ∀ (s : State),
           apply And.intro
           · simp [UInt256_ofNat_1]
           · simp [Stack.push]
-            rw [Sat256.natSub_zero]
 
 /-
  -   Comparison and Bitwise Logic Operations
@@ -698,7 +685,7 @@ theorem step_lt : ∀ (s : State),
         else
         .ok ({s with
                   machineState.stack := UInt256.lt a b :: t,
-                  machineState.gasAvailable := s.machineState.gasAvailable.natSub GasConstants.Gverylow
+                  machineState.gasAvailable := s.machineState.gasAvailable.subNat GasConstants.Gverylow
                   machineState.pc := s.machineState.pc + ⟨1⟩
                   machineState.execLength := s.machineState.execLength + 1
                   }
@@ -735,7 +722,6 @@ theorem step_lt : ∀ (s : State),
           apply And.intro
           · simp [UInt256_ofNat_1]
           · simp [Stack.push]
-            rw [Sat256.natSub_zero]
 
 theorem step_gt : ∀ (s : State),
   let I_b := s.executionEnv.code
@@ -749,7 +735,7 @@ theorem step_gt : ∀ (s : State),
         else
         .ok ({s with
                   machineState.stack := UInt256.gt a b :: t,
-                  machineState.gasAvailable := s.machineState.gasAvailable.natSub GasConstants.Gverylow
+                  machineState.gasAvailable := s.machineState.gasAvailable.subNat GasConstants.Gverylow
                   machineState.pc := s.machineState.pc + ⟨1⟩
                   machineState.execLength := s.machineState.execLength + 1
                   }
@@ -786,7 +772,6 @@ theorem step_gt : ∀ (s : State),
           apply And.intro
           · simp [UInt256_ofNat_1]
           · simp [Stack.push]
-            rw [Sat256.natSub_zero]
 
 theorem step_slt : ∀ (s : State),
   let I_b := s.executionEnv.code
@@ -800,7 +785,7 @@ theorem step_slt : ∀ (s : State),
         else
         .ok ({s with
                   machineState.stack := UInt256.slt a b :: t,
-                  machineState.gasAvailable := s.machineState.gasAvailable.natSub GasConstants.Gverylow
+                  machineState.gasAvailable := s.machineState.gasAvailable.subNat GasConstants.Gverylow
                   machineState.pc := s.machineState.pc + ⟨1⟩
                   machineState.execLength := s.machineState.execLength + 1
                   }
@@ -837,7 +822,6 @@ theorem step_slt : ∀ (s : State),
           apply And.intro
           · simp [UInt256_ofNat_1]
           · simp [Stack.push]
-            rw [Sat256.natSub_zero]
 
 theorem step_sgt : ∀ (s : State),
   let I_b := s.executionEnv.code
@@ -851,7 +835,7 @@ theorem step_sgt : ∀ (s : State),
         else
         .ok ({s with
                   machineState.stack := UInt256.sgt a b :: t,
-                  machineState.gasAvailable := s.machineState.gasAvailable.natSub GasConstants.Gverylow
+                  machineState.gasAvailable := s.machineState.gasAvailable.subNat GasConstants.Gverylow
                   machineState.pc := s.machineState.pc + ⟨1⟩
                   machineState.execLength := s.machineState.execLength + 1
                   }
@@ -888,7 +872,6 @@ theorem step_sgt : ∀ (s : State),
           apply And.intro
           · simp [UInt256_ofNat_1]
           · simp [Stack.push]
-            rw [Sat256.natSub_zero]
 
 theorem step_eq : ∀ (s : State),
   let I_b := s.executionEnv.code
@@ -902,7 +885,7 @@ theorem step_eq : ∀ (s : State),
         else
         .ok ({s with
                   machineState.stack := UInt256.eq a b :: t,
-                  machineState.gasAvailable := s.machineState.gasAvailable.natSub GasConstants.Gverylow
+                  machineState.gasAvailable := s.machineState.gasAvailable.subNat GasConstants.Gverylow
                   machineState.pc := s.machineState.pc + ⟨1⟩
                   machineState.execLength := s.machineState.execLength + 1
                   }
@@ -939,7 +922,6 @@ theorem step_eq : ∀ (s : State),
           apply And.intro
           · simp [UInt256_ofNat_1]
           · simp [Stack.push]
-            rw [Sat256.natSub_zero]
 
 theorem step_and : ∀ (s : State),
   let I_b := s.executionEnv.code
@@ -953,7 +935,7 @@ theorem step_and : ∀ (s : State),
         else
         .ok ({s with
                   machineState.stack := UInt256.land a b :: t,
-                  machineState.gasAvailable := s.machineState.gasAvailable.natSub GasConstants.Gverylow
+                  machineState.gasAvailable := s.machineState.gasAvailable.subNat GasConstants.Gverylow
                   machineState.pc := s.machineState.pc + ⟨1⟩
                   machineState.execLength := s.machineState.execLength + 1
                   }
@@ -990,7 +972,6 @@ theorem step_and : ∀ (s : State),
           apply And.intro
           · simp [UInt256_ofNat_1]
           · simp [Stack.push]
-            rw [Sat256.natSub_zero]
 
 theorem step_or : ∀ (s : State),
   let I_b := s.executionEnv.code
@@ -1004,7 +985,7 @@ theorem step_or : ∀ (s : State),
         else
         .ok ({s with
                   machineState.stack := UInt256.lor a b :: t,
-                  machineState.gasAvailable := s.machineState.gasAvailable.natSub GasConstants.Gverylow
+                  machineState.gasAvailable := s.machineState.gasAvailable.subNat GasConstants.Gverylow
                   machineState.pc := s.machineState.pc + ⟨1⟩
                   machineState.execLength := s.machineState.execLength + 1
                   }
@@ -1041,7 +1022,6 @@ theorem step_or : ∀ (s : State),
           apply And.intro
           · simp [UInt256_ofNat_1]
           · simp [Stack.push]
-            rw [Sat256.natSub_zero]
 
 theorem step_xor : ∀ (s : State),
   let I_b := s.executionEnv.code
@@ -1055,7 +1035,7 @@ theorem step_xor : ∀ (s : State),
         else
         .ok ({s with
                   machineState.stack := UInt256.xor a b :: t,
-                  machineState.gasAvailable := s.machineState.gasAvailable.natSub GasConstants.Gverylow
+                  machineState.gasAvailable := s.machineState.gasAvailable.subNat GasConstants.Gverylow
                   machineState.pc := s.machineState.pc + ⟨1⟩
                   machineState.execLength := s.machineState.execLength + 1
                   }
@@ -1092,7 +1072,6 @@ theorem step_xor : ∀ (s : State),
           apply And.intro
           · simp [UInt256_ofNat_1]
           · simp [Stack.push]
-            rw [Sat256.natSub_zero]
 
 theorem step_byte : ∀ (s : State),
   let I_b := s.executionEnv.code
@@ -1106,7 +1085,7 @@ theorem step_byte : ∀ (s : State),
         else
         .ok ({s with
                   machineState.stack := UInt256.byteAt a b :: t,
-                  machineState.gasAvailable := s.machineState.gasAvailable.natSub GasConstants.Gverylow
+                  machineState.gasAvailable := s.machineState.gasAvailable.subNat GasConstants.Gverylow
                   machineState.pc := s.machineState.pc + ⟨1⟩
                   machineState.execLength := s.machineState.execLength + 1
                   }
@@ -1143,7 +1122,6 @@ theorem step_byte : ∀ (s : State),
           apply And.intro
           · simp [UInt256_ofNat_1]
           · simp [Stack.push]
-            rw [Sat256.natSub_zero]
 
 theorem step_shl : ∀ (s : State),
   let I_b := s.executionEnv.code
@@ -1157,7 +1135,7 @@ theorem step_shl : ∀ (s : State),
         else
         .ok ({s with
                   machineState.stack := UInt256.shiftLeft b a :: t,
-                  machineState.gasAvailable := s.machineState.gasAvailable.natSub GasConstants.Gverylow
+                  machineState.gasAvailable := s.machineState.gasAvailable.subNat GasConstants.Gverylow
                   machineState.pc := s.machineState.pc + ⟨1⟩
                   machineState.execLength := s.machineState.execLength + 1
                   }
@@ -1194,7 +1172,6 @@ theorem step_shl : ∀ (s : State),
           apply And.intro
           · simp [UInt256_ofNat_1]
           · simp [Stack.push, flip]
-            rw [Sat256.natSub_zero]
 
 theorem step_shr : ∀ (s : State),
   let I_b := s.executionEnv.code
@@ -1208,7 +1185,7 @@ theorem step_shr : ∀ (s : State),
         else
         .ok ({s with
                   machineState.stack := UInt256.shiftRight b a :: t,
-                  machineState.gasAvailable := s.machineState.gasAvailable.natSub GasConstants.Gverylow
+                  machineState.gasAvailable := s.machineState.gasAvailable.subNat GasConstants.Gverylow
                   machineState.pc := s.machineState.pc + ⟨1⟩
                   machineState.execLength := s.machineState.execLength + 1
                   }
@@ -1245,7 +1222,6 @@ theorem step_shr : ∀ (s : State),
           apply And.intro
           · simp [UInt256_ofNat_1]
           · simp [Stack.push, flip]
-            rw [Sat256.natSub_zero]
 
 theorem step_sar : ∀ (s : State),
   let I_b := s.executionEnv.code
@@ -1259,7 +1235,7 @@ theorem step_sar : ∀ (s : State),
         else
         .ok ({s with
                   machineState.stack := UInt256.sar a b :: t,
-                  machineState.gasAvailable := s.machineState.gasAvailable.natSub GasConstants.Gverylow
+                  machineState.gasAvailable := s.machineState.gasAvailable.subNat GasConstants.Gverylow
                   machineState.pc := s.machineState.pc + ⟨1⟩
                   machineState.execLength := s.machineState.execLength + 1
                   }
@@ -1296,7 +1272,6 @@ theorem step_sar : ∀ (s : State),
           apply And.intro
           · simp [UInt256_ofNat_1]
           · simp [Stack.push]
-            rw [Sat256.natSub_zero]
 
 theorem step_iszero : ∀ (s : State),
   let I_b := s.executionEnv.code
@@ -1310,7 +1285,7 @@ theorem step_iszero : ∀ (s : State),
         else
         .ok ({s with
                   machineState.stack := UInt256.isZero a :: t,
-                  machineState.gasAvailable := s.machineState.gasAvailable.natSub GasConstants.Gverylow
+                  machineState.gasAvailable := s.machineState.gasAvailable.subNat GasConstants.Gverylow
                   machineState.pc := s.machineState.pc + ⟨1⟩
                   machineState.execLength := s.machineState.execLength + 1
                   }
@@ -1346,7 +1321,6 @@ theorem step_iszero : ∀ (s : State),
           apply And.intro
           · simp [UInt256_ofNat_1]
           · simp [Stack.push]
-            rw [Sat256.natSub_zero]
 
 theorem step_not : ∀ (s : State),
   let I_b := s.executionEnv.code
@@ -1360,7 +1334,7 @@ theorem step_not : ∀ (s : State),
         else
         .ok ({s with
                   machineState.stack := UInt256.lnot a :: t,
-                  machineState.gasAvailable := s.machineState.gasAvailable.natSub GasConstants.Gverylow
+                  machineState.gasAvailable := s.machineState.gasAvailable.subNat GasConstants.Gverylow
                   machineState.pc := s.machineState.pc + ⟨1⟩
                   machineState.execLength := s.machineState.execLength + 1
                   }
@@ -1396,7 +1370,6 @@ theorem step_not : ∀ (s : State),
           apply And.intro
           · simp [UInt256_ofNat_1]
           · simp [Stack.push]
-            rw [Sat256.natSub_zero]
 
 /-
  -   Keccak Operation
@@ -1411,7 +1384,7 @@ theorem step_keccak : ∀ (s : State),
         let memoryCost := memoryExpansionCost s .KECCAK256
         if s.machineState.gasAvailable.toNat < memoryCost then .error .OutOfGass
         else
-        let gasAvailable' := s.machineState.gasAvailable.natSub memoryCost
+        let gasAvailable' := s.machineState.gasAvailable.subNat memoryCost
         let hashCost := GasConstants.Gkeccak256 + GasConstants.Gkeccak256word * ((b.toNat + 31) / 32)
         if gasAvailable'.toNat < hashCost then .error .OutOfGass
         else
@@ -1421,7 +1394,7 @@ theorem step_keccak : ∀ (s : State),
         let kec := ffi.KEC bytes
         .ok ({s with
                   machineState.stack := UInt256.ofNat (fromByteArrayBigEndian kec) :: t,
-                  machineState.gasAvailable := gasAvailable'.natSub hashCost
+                  machineState.gasAvailable := gasAvailable'.subNat hashCost
                   machineState.pc := s.machineState.pc + ⟨1⟩
                   machineState.execLength := s.machineState.execLength + 1
                   machineState.activeWords :=
@@ -1441,28 +1414,28 @@ theorem step_keccak : ∀ (s : State),
       by_cases hmem : s.machineState.gasAvailable.toNat < memoryExpansionCost s .KECCAK256
       · simp [hmem]
       · simp [hmem]
-        let gasAvailable' := s.machineState.gasAvailable.natSub (memoryExpansionCost s .KECCAK256)
+        let gasAvailable' := s.machineState.gasAvailable.subNat (memoryExpansionCost s .KECCAK256)
         by_cases hgas :
             gasAvailable'.toNat <
               GasConstants.Gkeccak256 + GasConstants.Gkeccak256word * ((b.toNat + 31) / 32)
         · have hgas' :
-              (s.machineState.gasAvailable.natSub
+              (s.machineState.gasAvailable.subNat
                     (Cₘ (UInt256.ofNat
                         (MachineState.M s.machineState.activeWords.toNat a.toNat b.toNat)) -
                         Cₘ s.machineState.activeWords)).toNat <
                 GasConstants.Gkeccak256 + GasConstants.Gkeccak256word * ((b.toNat + 31) / 32) := by
             simpa [gasAvailable', memoryExpansionCost, memoryExpansionCost.μᵢ', hstack] using hgas
-          simp only [Sat256.natSub_toNat] at hgas'
+          simp only [Sat256.subNat_toNat] at hgas'
           simp [gasAvailable', hgas', memoryExpansionCost, memoryExpansionCost.μᵢ', C', hstack]
         ·
           have hgas' :
-              ¬ (s.machineState.gasAvailable.natSub
+              ¬ (s.machineState.gasAvailable.subNat
                     (Cₘ (UInt256.ofNat
                         (MachineState.M s.machineState.activeWords.toNat a.toNat b.toNat)) -
                         Cₘ s.machineState.activeWords)).toNat <
                 GasConstants.Gkeccak256 + GasConstants.Gkeccak256word * ((b.toNat + 31) / 32) := by
             simpa [gasAvailable', memoryExpansionCost, memoryExpansionCost.μᵢ', hstack] using hgas
-          simp only [Sat256.natSub_toNat] at hgas'
+          simp only [Sat256.subNat_toNat] at hgas'
           simp [gasAvailable', hgas', memoryExpansionCost, memoryExpansionCost.μᵢ', C', hstack]
           simp [α, Operation.isCreate]
           by_cases hoverflow : 1024 < t.length + 1
@@ -1494,7 +1467,7 @@ theorem step_address : ∀ (s : State),
       else
       .ok ({s with
                 machineState.stack := UInt256.ofNat s.executionEnv.codeOwner.val :: s.machineState.stack,
-                machineState.gasAvailable := s.machineState.gasAvailable.natSub GasConstants.Gbase
+                machineState.gasAvailable := s.machineState.gasAvailable.subNat GasConstants.Gbase
                 machineState.pc := s.machineState.pc + ⟨1⟩
                 machineState.execLength := s.machineState.execLength + 1
                 }
@@ -1520,7 +1493,6 @@ theorem step_address : ∀ (s : State),
         apply And.intro
         · simp [UInt256_ofNat_1]
         · simp [Stack.push, Ethereum.State.selfbalance]
-          rw [Sat256.natSub_zero]
 
 theorem step_origin : ∀ (s : State),
   let I_b := s.executionEnv.code
@@ -1532,7 +1504,7 @@ theorem step_origin : ∀ (s : State),
       else
       .ok ({s with
                 machineState.stack := UInt256.ofNat s.executionEnv.sender.val :: s.machineState.stack,
-                machineState.gasAvailable := s.machineState.gasAvailable.natSub GasConstants.Gbase
+                machineState.gasAvailable := s.machineState.gasAvailable.subNat GasConstants.Gbase
                 machineState.pc := s.machineState.pc + ⟨1⟩
                 machineState.execLength := s.machineState.execLength + 1
                 }
@@ -1558,7 +1530,6 @@ theorem step_origin : ∀ (s : State),
         apply And.intro
         · simp [UInt256_ofNat_1]
         · simp [Stack.push]
-          rw [Sat256.natSub_zero]
 
 theorem step_caller : ∀ (s : State),
   let I_b := s.executionEnv.code
@@ -1570,7 +1541,7 @@ theorem step_caller : ∀ (s : State),
       else
       .ok ({s with
                 machineState.stack := UInt256.ofNat s.executionEnv.source.val :: s.machineState.stack,
-                machineState.gasAvailable := s.machineState.gasAvailable.natSub GasConstants.Gbase
+                machineState.gasAvailable := s.machineState.gasAvailable.subNat GasConstants.Gbase
                 machineState.pc := s.machineState.pc + ⟨1⟩
                 machineState.execLength := s.machineState.execLength + 1
                 }
@@ -1596,7 +1567,6 @@ theorem step_caller : ∀ (s : State),
         apply And.intro
         · simp [UInt256_ofNat_1]
         · simp [Stack.push]
-          rw [Sat256.natSub_zero]
 
 theorem step_callvalue : ∀ (s : State),
   let I_b := s.executionEnv.code
@@ -1608,7 +1578,7 @@ theorem step_callvalue : ∀ (s : State),
       else
       .ok ({s with
                 machineState.stack := s.executionEnv.weiValue :: s.machineState.stack,
-                machineState.gasAvailable := s.machineState.gasAvailable.natSub GasConstants.Gbase
+                machineState.gasAvailable := s.machineState.gasAvailable.subNat GasConstants.Gbase
                 machineState.pc := s.machineState.pc + ⟨1⟩
                 machineState.execLength := s.machineState.execLength + 1
                 }
@@ -1634,7 +1604,6 @@ theorem step_callvalue : ∀ (s : State),
         apply And.intro
         · simp [UInt256_ofNat_1]
         · simp [Stack.push]
-          rw [Sat256.natSub_zero]
 
 theorem step_calldatasize : ∀ (s : State),
   let I_b := s.executionEnv.code
@@ -1646,7 +1615,7 @@ theorem step_calldatasize : ∀ (s : State),
       else
       .ok ({s with
                 machineState.stack := UInt256.ofNat s.executionEnv.calldata.size :: s.machineState.stack,
-                machineState.gasAvailable := s.machineState.gasAvailable.natSub GasConstants.Gbase
+                machineState.gasAvailable := s.machineState.gasAvailable.subNat GasConstants.Gbase
                 machineState.pc := s.machineState.pc + ⟨1⟩
                 machineState.execLength := s.machineState.execLength + 1
                 }
@@ -1672,7 +1641,6 @@ theorem step_calldatasize : ∀ (s : State),
         apply And.intro
         · simp [UInt256_ofNat_1]
         · simp [Stack.push]
-          rw [Sat256.natSub_zero]
 
 theorem step_codesize : ∀ (s : State),
   let I_b := s.executionEnv.code
@@ -1684,7 +1652,7 @@ theorem step_codesize : ∀ (s : State),
       else
       .ok ({s with
                 machineState.stack := UInt256.ofNat s.executionEnv.code.size :: s.machineState.stack,
-                machineState.gasAvailable := s.machineState.gasAvailable.natSub GasConstants.Gbase
+                machineState.gasAvailable := s.machineState.gasAvailable.subNat GasConstants.Gbase
                 machineState.pc := s.machineState.pc + ⟨1⟩
                 machineState.execLength := s.machineState.execLength + 1
                 }
@@ -1710,7 +1678,6 @@ theorem step_codesize : ∀ (s : State),
         apply And.intro
         · simp [UInt256_ofNat_1]
         · simp [Stack.push]
-          rw [Sat256.natSub_zero]
 
 theorem step_gasprice : ∀ (s : State),
   let I_b := s.executionEnv.code
@@ -1722,7 +1689,7 @@ theorem step_gasprice : ∀ (s : State),
       else
       .ok ({s with
                 machineState.stack := UInt256.ofNat s.executionEnv.gasPrice :: s.machineState.stack,
-                machineState.gasAvailable := s.machineState.gasAvailable.natSub GasConstants.Gbase
+                machineState.gasAvailable := s.machineState.gasAvailable.subNat GasConstants.Gbase
                 machineState.pc := s.machineState.pc + ⟨1⟩
                 machineState.execLength := s.machineState.execLength + 1
                 }
@@ -1748,7 +1715,6 @@ theorem step_gasprice : ∀ (s : State),
         apply And.intro
         · simp [UInt256_ofNat_1]
         · simp [Stack.push]
-          rw [Sat256.natSub_zero]
 
 theorem step_returndatasize : ∀ (s : State),
   let I_b := s.executionEnv.code
@@ -1760,7 +1726,7 @@ theorem step_returndatasize : ∀ (s : State),
       else
       .ok ({s with
                 machineState.stack := UInt256.ofNat s.machineState.returnData.size :: s.machineState.stack,
-                machineState.gasAvailable := s.machineState.gasAvailable.natSub GasConstants.Gbase
+                machineState.gasAvailable := s.machineState.gasAvailable.subNat GasConstants.Gbase
                 machineState.pc := s.machineState.pc + ⟨1⟩
                 machineState.execLength := s.machineState.execLength + 1
                 }
@@ -1786,7 +1752,6 @@ theorem step_returndatasize : ∀ (s : State),
         apply And.intro
         · simp [UInt256_ofNat_1]
         · simp [Stack.push]
-          rw [Sat256.natSub_zero]
 
 theorem step_coinbase : ∀ (s : State),
   let I_b := s.executionEnv.code
@@ -1798,7 +1763,7 @@ theorem step_coinbase : ∀ (s : State),
       else
       .ok ({s with
                 machineState.stack := UInt256.ofNat s.executionEnv.header.beneficiary.val :: s.machineState.stack,
-                machineState.gasAvailable := s.machineState.gasAvailable.natSub GasConstants.Gbase
+                machineState.gasAvailable := s.machineState.gasAvailable.subNat GasConstants.Gbase
                 machineState.pc := s.machineState.pc + ⟨1⟩
                 machineState.execLength := s.machineState.execLength + 1
                 }
@@ -1824,7 +1789,6 @@ theorem step_coinbase : ∀ (s : State),
         apply And.intro
         · simp [UInt256_ofNat_1]
         · simp [Stack.push]
-          rw [Sat256.natSub_zero]
 
 theorem step_timestamp : ∀ (s : State),
   let I_b := s.executionEnv.code
@@ -1836,7 +1800,7 @@ theorem step_timestamp : ∀ (s : State),
       else
       .ok ({s with
                 machineState.stack := UInt256.ofNat s.executionEnv.header.timestamp :: s.machineState.stack,
-                machineState.gasAvailable := s.machineState.gasAvailable.natSub GasConstants.Gbase
+                machineState.gasAvailable := s.machineState.gasAvailable.subNat GasConstants.Gbase
                 machineState.pc := s.machineState.pc + ⟨1⟩
                 machineState.execLength := s.machineState.execLength + 1
                 }
@@ -1862,7 +1826,6 @@ theorem step_timestamp : ∀ (s : State),
         apply And.intro
         · simp [UInt256_ofNat_1]
         · simp [Stack.push]
-          rw [Sat256.natSub_zero]
 
 theorem step_number : ∀ (s : State),
   let I_b := s.executionEnv.code
@@ -1874,7 +1837,7 @@ theorem step_number : ∀ (s : State),
       else
       .ok ({s with
                 machineState.stack := UInt256.ofNat s.executionEnv.header.number :: s.machineState.stack,
-                machineState.gasAvailable := s.machineState.gasAvailable.natSub GasConstants.Gbase
+                machineState.gasAvailable := s.machineState.gasAvailable.subNat GasConstants.Gbase
                 machineState.pc := s.machineState.pc + ⟨1⟩
                 machineState.execLength := s.machineState.execLength + 1
                 }
@@ -1900,7 +1863,6 @@ theorem step_number : ∀ (s : State),
         apply And.intro
         · simp [UInt256_ofNat_1]
         · simp [Stack.push]
-          rw [Sat256.natSub_zero]
 
 theorem step_prevrandao : ∀ (s : State),
   let I_b := s.executionEnv.code
@@ -1912,7 +1874,7 @@ theorem step_prevrandao : ∀ (s : State),
       else
       .ok ({s with
                 machineState.stack := s.executionEnv.header.prevRandao :: s.machineState.stack,
-                machineState.gasAvailable := s.machineState.gasAvailable.natSub GasConstants.Gbase
+                machineState.gasAvailable := s.machineState.gasAvailable.subNat GasConstants.Gbase
                 machineState.pc := s.machineState.pc + ⟨1⟩
                 machineState.execLength := s.machineState.execLength + 1
                 }
@@ -1938,7 +1900,6 @@ theorem step_prevrandao : ∀ (s : State),
         apply And.intro
         · simp [UInt256_ofNat_1]
         · simp [Stack.push]
-          rw [Sat256.natSub_zero]
 
 theorem step_gaslimit : ∀ (s : State),
   let I_b := s.executionEnv.code
@@ -1950,7 +1911,7 @@ theorem step_gaslimit : ∀ (s : State),
       else
       .ok ({s with
                 machineState.stack := UInt256.ofNat s.executionEnv.header.gasLimit :: s.machineState.stack,
-                machineState.gasAvailable := s.machineState.gasAvailable.natSub GasConstants.Gbase
+                machineState.gasAvailable := s.machineState.gasAvailable.subNat GasConstants.Gbase
                 machineState.pc := s.machineState.pc + ⟨1⟩
                 machineState.execLength := s.machineState.execLength + 1
                 }
@@ -1976,7 +1937,6 @@ theorem step_gaslimit : ∀ (s : State),
         apply And.intro
         · simp [UInt256_ofNat_1]
         · simp [Stack.push]
-          rw [Sat256.natSub_zero]
 
 theorem step_chainid : ∀ (s : State),
   let I_b := s.executionEnv.code
@@ -1988,7 +1948,7 @@ theorem step_chainid : ∀ (s : State),
       else
       .ok ({s with
                 machineState.stack := UInt256.ofNat Ethereum.chainId :: s.machineState.stack,
-                machineState.gasAvailable := s.machineState.gasAvailable.natSub GasConstants.Gbase
+                machineState.gasAvailable := s.machineState.gasAvailable.subNat GasConstants.Gbase
                 machineState.pc := s.machineState.pc + ⟨1⟩
                 machineState.execLength := s.machineState.execLength + 1
                 }
@@ -2014,7 +1974,6 @@ theorem step_chainid : ∀ (s : State),
         apply And.intro
         · simp [UInt256_ofNat_1]
         · simp [Stack.push]
-          rw [Sat256.natSub_zero]
 
 theorem step_basefee : ∀ (s : State),
   let I_b := s.executionEnv.code
@@ -2026,7 +1985,7 @@ theorem step_basefee : ∀ (s : State),
       else
       .ok ({s with
                 machineState.stack := UInt256.ofNat s.executionEnv.header.baseFeePerGas :: s.machineState.stack,
-                machineState.gasAvailable := s.machineState.gasAvailable.natSub GasConstants.Gbase
+                machineState.gasAvailable := s.machineState.gasAvailable.subNat GasConstants.Gbase
                 machineState.pc := s.machineState.pc + ⟨1⟩
                 machineState.execLength := s.machineState.execLength + 1
                 }
@@ -2052,7 +2011,6 @@ theorem step_basefee : ∀ (s : State),
         apply And.intro
         · simp [UInt256_ofNat_1]
         · simp [Stack.push]
-          rw [Sat256.natSub_zero]
 
 theorem step_blobbasefee : ∀ (s : State),
   let I_b := s.executionEnv.code
@@ -2064,7 +2022,7 @@ theorem step_blobbasefee : ∀ (s : State),
       else
       .ok ({s with
                 machineState.stack := UInt256.ofNat s.executionEnv.header.getBlobGasprice :: s.machineState.stack,
-                machineState.gasAvailable := s.machineState.gasAvailable.natSub GasConstants.Gbase
+                machineState.gasAvailable := s.machineState.gasAvailable.subNat GasConstants.Gbase
                 machineState.pc := s.machineState.pc + ⟨1⟩
                 machineState.execLength := s.machineState.execLength + 1
                 }
@@ -2090,7 +2048,6 @@ theorem step_blobbasefee : ∀ (s : State),
         apply And.intro
         · simp [UInt256_ofNat_1]
         · simp [Stack.push]
-          rw [Sat256.natSub_zero]
 
 theorem step_calldataload : ∀ (s : State),
   let I_b := s.executionEnv.code
@@ -2105,7 +2062,7 @@ theorem step_calldataload : ∀ (s : State),
         .ok ({s with
                   machineState.stack :=
                     (uInt256OfByteArray <| s.executionEnv.calldata.readBytes a.toNat 32) :: t,
-                  machineState.gasAvailable := s.machineState.gasAvailable.natSub GasConstants.Gverylow
+                  machineState.gasAvailable := s.machineState.gasAvailable.subNat GasConstants.Gverylow
                   machineState.pc := s.machineState.pc + ⟨1⟩
                   machineState.execLength := s.machineState.execLength + 1
                   }
@@ -2141,9 +2098,7 @@ theorem step_calldataload : ∀ (s : State),
           apply And.intro
           · simp [UInt256_ofNat_1]
           · simp [Stack.push]
-            apply And.intro
-            · simp [Ethereum.State.calldataload]
-            · rw [Sat256.natSub_zero]
+            simp [Ethereum.State.calldataload]
 
 theorem step_blockhash : ∀ (s : State),
   let I_b := s.executionEnv.code
@@ -2161,7 +2116,7 @@ theorem step_blockhash : ∀ (s : State),
                       ⟨0⟩
                     else
                       s.blocks.map ProcessedBlock.hash |>.getD a.toNat ⟨0⟩) :: t,
-                  machineState.gasAvailable := s.machineState.gasAvailable.natSub GasConstants.Gblockhash
+                  machineState.gasAvailable := s.machineState.gasAvailable.subNat GasConstants.Gblockhash
                   machineState.pc := s.machineState.pc + ⟨1⟩
                   machineState.execLength := s.machineState.execLength + 1
                   }
@@ -2191,9 +2146,7 @@ theorem step_blockhash : ∀ (s : State),
           apply And.intro
           · simp [UInt256_ofNat_1]
           · simp [Stack.push]
-            apply And.intro
-            · simp [Ethereum.State.blockHash, Ethereum.State.blockHashes]
-            · rw [Sat256.natSub_zero]
+            simp [Ethereum.State.blockHash, Ethereum.State.blockHashes]
 
 theorem step_blobhash : ∀ (s : State),
   let I_b := s.executionEnv.code
@@ -2209,7 +2162,7 @@ theorem step_blobhash : ∀ (s : State),
                   machineState.stack :=
                     (s.executionEnv.blobVersionedHashes[a.toNat]?.option ⟨0⟩
                       (.ofNat ∘ fromByteArrayBigEndian)) :: t,
-                  machineState.gasAvailable := s.machineState.gasAvailable.natSub GasConstants.HASH_OPCODE_GAS
+                  machineState.gasAvailable := s.machineState.gasAvailable.subNat GasConstants.HASH_OPCODE_GAS
                   machineState.pc := s.machineState.pc + ⟨1⟩
                   machineState.execLength := s.machineState.execLength + 1
                   }
@@ -2240,7 +2193,6 @@ theorem step_blobhash : ∀ (s : State),
           apply And.intro
           · simp [UInt256_ofNat_1]
           · simp [Stack.push]
-            rw [Sat256.natSub_zero]
 
 theorem step_selfbalance : ∀ (s : State),
   let I_b := s.executionEnv.code
@@ -2254,7 +2206,7 @@ theorem step_selfbalance : ∀ (s : State),
                 machineState.stack :=
                   (s.accountMap.find? s.executionEnv.codeOwner |>.elim ⟨0⟩ (·.balance)) ::
                     s.machineState.stack,
-                machineState.gasAvailable := s.machineState.gasAvailable.natSub GasConstants.Glow
+                machineState.gasAvailable := s.machineState.gasAvailable.subNat GasConstants.Glow
                 machineState.pc := s.machineState.pc + ⟨1⟩
                 machineState.execLength := s.machineState.execLength + 1
                 }
@@ -2285,9 +2237,8 @@ theorem step_selfbalance : ∀ (s : State),
         apply And.intro
         · simp [UInt256_ofNat_1]
         · simp [Stack.push]
-          apply And.intro
-          · simp [Ethereum.State.selfbalance]
-          · rw [Sat256.natSub_zero]
+          simp [Ethereum.State.selfbalance]
+
 theorem step_balance : ∀ (s : State),
   let I_b := s.executionEnv.code
   decode I_b s.machineState.pc = some (.BALANCE, .none)
@@ -2305,7 +2256,7 @@ theorem step_balance : ∀ (s : State),
                     {s.substate with
                       accessedAccounts := s.substate.accessedAccounts.insert addr}
                   machineState.stack := (s.accountMap.find? addr |>.elim ⟨0⟩ (·.balance)) :: t,
-                  machineState.gasAvailable := s.machineState.gasAvailable.natSub gasCost
+                  machineState.gasAvailable := s.machineState.gasAvailable.subNat gasCost
                   machineState.pc := s.machineState.pc + ⟨1⟩
                   machineState.execLength := s.machineState.execLength + 1
                   }
@@ -2339,9 +2290,7 @@ theorem step_balance : ∀ (s : State),
           · simp [Ethereum.State.balance, Ethereum.State.addAccessedAccount]
           · simp [Stack.push, Ethereum.State.balance, Ethereum.State.addAccessedAccount,
               Ethereum.Substate.addAccessedAccount]
-            apply And.intro
-            · rw [UInt256_ofNat_1]
-            · rw [Sat256.natSub_zero]
+            rw [UInt256_ofNat_1]
 
 theorem step_extcodesize : ∀ (s : State),
   let I_b := s.executionEnv.code
@@ -2361,7 +2310,7 @@ theorem step_extcodesize : ∀ (s : State),
                       accessedAccounts := s.substate.accessedAccounts.insert addr}
                   machineState.stack :=
                     (s.accountMap.find? addr |>.option ⟨0⟩ (.ofNat ∘ ByteArray.size ∘ (·.code))) :: t,
-                  machineState.gasAvailable := s.machineState.gasAvailable.natSub gasCost
+                  machineState.gasAvailable := s.machineState.gasAvailable.subNat gasCost
                   machineState.pc := s.machineState.pc + ⟨1⟩
                   machineState.execLength := s.machineState.execLength + 1
                   }
@@ -2396,9 +2345,7 @@ theorem step_extcodesize : ∀ (s : State),
               Ethereum.State.addAccessedAccount]
           · simp [Stack.push, Ethereum.State.extCodeSize, Ethereum.State.lookupAccount,
               Ethereum.State.addAccessedAccount, Ethereum.Substate.addAccessedAccount]
-            apply And.intro
-            · rw [UInt256_ofNat_1]
-            · rw [Sat256.natSub_zero]
+            rw [UInt256_ofNat_1]
 
 theorem step_extcodehash : ∀ (s : State),
   let I_b := s.executionEnv.code
@@ -2422,7 +2369,7 @@ theorem step_extcodehash : ∀ (s : State),
                     {s.substate with
                       accessedAccounts := s.substate.accessedAccounts.insert addr}
                   machineState.stack := hash :: t
-                  machineState.gasAvailable := s.machineState.gasAvailable.natSub gasCost
+                  machineState.gasAvailable := s.machineState.gasAvailable.subNat gasCost
                   machineState.pc := s.machineState.pc + ⟨1⟩
                   machineState.execLength := s.machineState.execLength + 1
                   }
@@ -2453,12 +2400,12 @@ theorem step_extcodehash : ∀ (s : State),
           unfold Ethereum.State.incrPC
           simp [Stack.push, Ethereum.State.extCodeHash, Ethereum.State.dead,
             Ethereum.State.lookupAccount, Ethereum.State.addAccessedAccount,
-            Ethereum.Substate.addAccessedAccount, UInt256_ofNat_1, Sat256.natSub_zero, UInt256_subzero']
+            Ethereum.Substate.addAccessedAccount, UInt256_ofNat_1, Sat256.subNat_zero, UInt256_subzero']
           by_cases hdead :
               Option.option true Account.emptyAccount
                 (Batteries.RBMap.find? s.accountMap (AccountAddress.ofUInt256 a)) = true
-          · simp [hdead, UInt256_ofNat_1, Sat256.natSub_zero, UInt256_subzero']
-          · simp [hdead, UInt256_ofNat_1, Sat256.natSub_zero, UInt256_subzero']
+          · simp [hdead, UInt256_ofNat_1, Sat256.subNat_zero, UInt256_subzero']
+          · simp [hdead, UInt256_ofNat_1, Sat256.subNat_zero, UInt256_subzero']
 
 /-
  -   Machine and Stack Operations
@@ -2476,7 +2423,7 @@ theorem step_pop : ∀ (s : State),
         else
         .ok ({s with
                   machineState.stack := t,
-                  machineState.gasAvailable := s.machineState.gasAvailable.natSub GasConstants.Gbase
+                  machineState.gasAvailable := s.machineState.gasAvailable.subNat GasConstants.Gbase
                   machineState.pc := s.machineState.pc + ⟨1⟩
                   machineState.execLength := s.machineState.execLength + 1
                   }
@@ -2505,9 +2452,8 @@ theorem step_pop : ∀ (s : State),
           simp [Stack.pop, Ethereum.State.replaceStackAndIncrPC]
           unfold Ethereum.State.incrPC
           simp
-          apply And.intro
-          · simp [UInt256_ofNat_1]
-          · rw [Sat256.natSub_zero]
+          simp [UInt256_ofNat_1]
+
 theorem step_mload : ∀ (s : State),
   let I_b := s.executionEnv.code
   decode I_b s.machineState.pc = some (.MLOAD, .none)
@@ -2517,7 +2463,7 @@ theorem step_mload : ∀ (s : State),
         let memoryCost := memoryExpansionCost s .MLOAD
         if s.machineState.gasAvailable.toNat < memoryCost then .error .OutOfGass
         else
-        let gasAvailable' := s.machineState.gasAvailable.natSub memoryCost
+        let gasAvailable' := s.machineState.gasAvailable.subNat memoryCost
         if gasAvailable'.toNat < GasConstants.Gverylow then .error .OutOfGass
         else
         if s.machineState.stack.length - 1 + 1 > 1024 then .error .StackOverflow
@@ -2533,7 +2479,7 @@ theorem step_mload : ∀ (s : State),
                           (s.machineState.memory.readWithPadding a.toNat 32))) :: t
                   machineState.activeWords :=
                     UInt256.ofNat (MachineState.M s.machineState.activeWords.toNat a.toNat 32)
-                  machineState.gasAvailable := gasAvailable'.natSub GasConstants.Gverylow
+                  machineState.gasAvailable := gasAvailable'.subNat GasConstants.Gverylow
                   machineState.pc := s.machineState.pc + ⟨1⟩
                   machineState.execLength := s.machineState.execLength + 1
                   }
@@ -2550,29 +2496,29 @@ theorem step_mload : ∀ (s : State),
       by_cases hmem : s.machineState.gasAvailable.toNat < memoryExpansionCost s .MLOAD
       · simp [hmem]
       · simp [hmem]
-        let gasAvailable' := s.machineState.gasAvailable.natSub (memoryExpansionCost s .MLOAD)
+        let gasAvailable' := s.machineState.gasAvailable.subNat (memoryExpansionCost s .MLOAD)
         by_cases hgas : gasAvailable'.toNat < GasConstants.Gverylow
         · have hgas' :
-              (s.machineState.gasAvailable.natSub
+              (s.machineState.gasAvailable.subNat
                     (Cₘ (UInt256.ofNat
                         (MachineState.M s.machineState.activeWords.toNat a.toNat 32)) -
                         Cₘ s.machineState.activeWords)).toNat <
                 GasConstants.Gverylow := by
             simpa [gasAvailable', memoryExpansionCost, memoryExpansionCost.μᵢ', hstack] using hgas
-          simp only [Sat256.natSub_toNat] at hgas'
+          simp only [Sat256.subNat_toNat] at hgas'
           simp [gasAvailable', hgas', memoryExpansionCost, memoryExpansionCost.μᵢ', C', hstack,
             InstructionGasGroups.Wcopy, InstructionGasGroups.Wextaccount,
             InstructionGasGroups.Wzero, InstructionGasGroups.Wbase,
             InstructionGasGroups.Wverylow]
         ·
           have hgas' :
-              ¬ (s.machineState.gasAvailable.natSub
+              ¬ (s.machineState.gasAvailable.subNat
                     (Cₘ (UInt256.ofNat
                         (MachineState.M s.machineState.activeWords.toNat a.toNat 32)) -
                         Cₘ s.machineState.activeWords)).toNat <
                 GasConstants.Gverylow := by
             simpa [gasAvailable', memoryExpansionCost, memoryExpansionCost.μᵢ', hstack] using hgas
-          simp only [Sat256.natSub_toNat] at hgas'
+          simp only [Sat256.subNat_toNat] at hgas'
           simp [gasAvailable', hgas', memoryExpansionCost, memoryExpansionCost.μᵢ', C', hstack,
             InstructionGasGroups.Wcopy, InstructionGasGroups.Wextaccount,
             InstructionGasGroups.Wzero, InstructionGasGroups.Wbase,
@@ -2600,7 +2546,7 @@ theorem step_mstore : ∀ (s : State),
         let memoryCost := memoryExpansionCost s .MSTORE
         if s.machineState.gasAvailable.toNat < memoryCost then .error .OutOfGass
         else
-        let gasAvailable' := s.machineState.gasAvailable.natSub memoryCost
+        let gasAvailable' := s.machineState.gasAvailable.subNat memoryCost
         if gasAvailable'.toNat < GasConstants.Gverylow then .error .OutOfGass
         else
         if s.machineState.stack.length - 2 + 0 > 1024 then .error .StackOverflow
@@ -2610,7 +2556,7 @@ theorem step_mstore : ∀ (s : State),
                   machineState.memory := b.toByteArray.write 0 s.machineState.memory a.toNat 32
                   machineState.activeWords :=
                     UInt256.ofNat (MachineState.M s.machineState.activeWords.toNat a.toNat 32)
-                  machineState.gasAvailable := gasAvailable'.natSub GasConstants.Gverylow
+                  machineState.gasAvailable := gasAvailable'.subNat GasConstants.Gverylow
                   machineState.pc := s.machineState.pc + ⟨1⟩
                   machineState.execLength := s.machineState.execLength + 1
                   }
@@ -2628,29 +2574,29 @@ theorem step_mstore : ∀ (s : State),
       by_cases hmem : s.machineState.gasAvailable.toNat < memoryExpansionCost s .MSTORE
       · simp [hmem]
       · simp [hmem]
-        let gasAvailable' := s.machineState.gasAvailable.natSub (memoryExpansionCost s .MSTORE)
+        let gasAvailable' := s.machineState.gasAvailable.subNat (memoryExpansionCost s .MSTORE)
         by_cases hgas : gasAvailable'.toNat < GasConstants.Gverylow
         · have hgas' :
-              (s.machineState.gasAvailable.natSub
+              (s.machineState.gasAvailable.subNat
                     (Cₘ (UInt256.ofNat
                         (MachineState.M s.machineState.activeWords.toNat a.toNat 32)) -
                         Cₘ s.machineState.activeWords)).toNat <
                 GasConstants.Gverylow := by
             simpa [gasAvailable', memoryExpansionCost, memoryExpansionCost.μᵢ', hstack] using hgas
-          simp only [Sat256.natSub_toNat] at hgas'
+          simp only [Sat256.subNat_toNat] at hgas'
           simp [gasAvailable', hgas', memoryExpansionCost, memoryExpansionCost.μᵢ', C', hstack,
             InstructionGasGroups.Wcopy, InstructionGasGroups.Wextaccount,
             InstructionGasGroups.Wzero, InstructionGasGroups.Wbase,
             InstructionGasGroups.Wverylow]
         ·
           have hgas' :
-              ¬ (s.machineState.gasAvailable.natSub
+              ¬ (s.machineState.gasAvailable.subNat
                     (Cₘ (UInt256.ofNat
                         (MachineState.M s.machineState.activeWords.toNat a.toNat 32)) -
                         Cₘ s.machineState.activeWords)).toNat <
                 GasConstants.Gverylow := by
             simpa [gasAvailable', memoryExpansionCost, memoryExpansionCost.μᵢ', hstack] using hgas
-          simp only [Sat256.natSub_toNat] at hgas'
+          simp only [Sat256.subNat_toNat] at hgas'
           simp [gasAvailable', hgas', memoryExpansionCost, memoryExpansionCost.μᵢ', C', hstack,
             InstructionGasGroups.Wcopy, InstructionGasGroups.Wextaccount,
             InstructionGasGroups.Wzero, InstructionGasGroups.Wbase,
@@ -2676,7 +2622,7 @@ theorem step_mstore8 : ∀ (s : State),
         let memoryCost := memoryExpansionCost s .MSTORE8
         if s.machineState.gasAvailable.toNat < memoryCost then .error .OutOfGass
         else
-        let gasAvailable' := s.machineState.gasAvailable.natSub memoryCost
+        let gasAvailable' := s.machineState.gasAvailable.subNat memoryCost
         if gasAvailable'.toNat < GasConstants.Gverylow then .error .OutOfGass
         else
         if s.machineState.stack.length - 2 + 0 > 1024 then .error .StackOverflow
@@ -2687,7 +2633,7 @@ theorem step_mstore8 : ∀ (s : State),
                     (⟨#[UInt8.ofNat b.toNat]⟩ : ByteArray).write 0 s.machineState.memory a.toNat 1
                   machineState.activeWords :=
                     UInt256.ofNat (MachineState.M s.machineState.activeWords.toNat a.toNat 1)
-                  machineState.gasAvailable := gasAvailable'.natSub GasConstants.Gverylow
+                  machineState.gasAvailable := gasAvailable'.subNat GasConstants.Gverylow
                   machineState.pc := s.machineState.pc + ⟨1⟩
                   machineState.execLength := s.machineState.execLength + 1
                   }
@@ -2705,29 +2651,29 @@ theorem step_mstore8 : ∀ (s : State),
       by_cases hmem : s.machineState.gasAvailable.toNat < memoryExpansionCost s .MSTORE8
       · simp [hmem]
       · simp [hmem]
-        let gasAvailable' := s.machineState.gasAvailable.natSub (memoryExpansionCost s .MSTORE8)
+        let gasAvailable' := s.machineState.gasAvailable.subNat (memoryExpansionCost s .MSTORE8)
         by_cases hgas : gasAvailable'.toNat < GasConstants.Gverylow
         · have hgas' :
-              (s.machineState.gasAvailable.natSub
+              (s.machineState.gasAvailable.subNat
                     (Cₘ (UInt256.ofNat
                         (MachineState.M s.machineState.activeWords.toNat a.toNat 1)) -
                         Cₘ s.machineState.activeWords)).toNat <
                 GasConstants.Gverylow := by
             simpa [gasAvailable', memoryExpansionCost, memoryExpansionCost.μᵢ', hstack] using hgas
-          simp only [Sat256.natSub_toNat] at hgas'
+          simp only [Sat256.subNat_toNat] at hgas'
           simp [gasAvailable', hgas', memoryExpansionCost, memoryExpansionCost.μᵢ', C', hstack,
             InstructionGasGroups.Wcopy, InstructionGasGroups.Wextaccount,
             InstructionGasGroups.Wzero, InstructionGasGroups.Wbase,
             InstructionGasGroups.Wverylow]
         ·
           have hgas' :
-              ¬ (s.machineState.gasAvailable.natSub
+              ¬ (s.machineState.gasAvailable.subNat
                     (Cₘ (UInt256.ofNat
                         (MachineState.M s.machineState.activeWords.toNat a.toNat 1)) -
                         Cₘ s.machineState.activeWords)).toNat <
                 GasConstants.Gverylow := by
             simpa [gasAvailable', memoryExpansionCost, memoryExpansionCost.μᵢ', hstack] using hgas
-          simp only [Sat256.natSub_toNat] at hgas'
+          simp only [Sat256.subNat_toNat] at hgas'
           simp [gasAvailable', hgas', memoryExpansionCost, memoryExpansionCost.μᵢ', C', hstack,
             InstructionGasGroups.Wcopy, InstructionGasGroups.Wextaccount,
             InstructionGasGroups.Wzero, InstructionGasGroups.Wbase,
@@ -2764,7 +2710,7 @@ theorem step_sload : ∀ (s : State),
                       accessedStorageKeys :=
                         s.substate.accessedStorageKeys.insert (s.executionEnv.codeOwner, a)}
                   machineState.stack := value :: t
-                  machineState.gasAvailable := s.machineState.gasAvailable.natSub gasCost
+                  machineState.gasAvailable := s.machineState.gasAvailable.subNat gasCost
                   machineState.pc := s.machineState.pc + ⟨1⟩
                   machineState.execLength := s.machineState.execLength + 1
                   }
@@ -2795,7 +2741,6 @@ theorem step_sload : ∀ (s : State),
           unfold Ethereum.State.incrPC
           simp [Ethereum.State.sload, Ethereum.State.lookupAccount, Ethereum.State.addAccessedStorageKey,
           Ethereum.Substate.addAccessedStorageKey, Account.lookupStorage, Stack.push, UInt256_ofNat_1]
-          rw [Sat256.natSub_zero]
 
 theorem step_tload : ∀ (s : State),
   let I_b := s.executionEnv.code
@@ -2812,7 +2757,7 @@ theorem step_tload : ∀ (s : State),
             (fun acc => acc.tstorage.findD a ⟨0⟩)
         .ok ({s with
                   machineState.stack := value :: t
-                  machineState.gasAvailable := s.machineState.gasAvailable.natSub Ctload
+                  machineState.gasAvailable := s.machineState.gasAvailable.subNat Ctload
                   machineState.pc := s.machineState.pc + ⟨1⟩
                   machineState.execLength := s.machineState.execLength + 1
                   }
@@ -2842,7 +2787,6 @@ theorem step_tload : ∀ (s : State),
           unfold Ethereum.State.incrPC
           simp [Ethereum.State.tload, Ethereum.State.lookupAccount, Account.lookupTransientStorage,
           Stack.push, UInt256_ofNat_1]
-          rw [Sat256.natSub_zero]
 
 theorem step_tstore : ∀ (s : State),
   let I_b := s.executionEnv.code
@@ -2865,7 +2809,7 @@ theorem step_tstore : ∀ (s : State),
         .ok ({s with
                   accountMap := accountMap
                   machineState.stack := t
-                  machineState.gasAvailable := s.machineState.gasAvailable.natSub Ctstore
+                  machineState.gasAvailable := s.machineState.gasAvailable.subNat Ctstore
                   machineState.pc := s.machineState.pc + ⟨1⟩
                   machineState.execLength := s.machineState.execLength + 1
                   }
@@ -2906,12 +2850,12 @@ theorem step_tstore : ∀ (s : State),
             | none =>
               simp [Ethereum.State.tstore, Ethereum.State.lookupAccount,
                 Ethereum.State.updateAccount, Account.updateTransientStorage,
-                Stack.push, UInt256_ofNat_1, Sat256.natSub_zero, UInt256_subzero', hacc, hperm,
+                Stack.push, UInt256_ofNat_1, Sat256.subNat_zero, UInt256_subzero', hacc, hperm,
                 Option.option]
             | some acc =>
               simp [Ethereum.State.tstore, Ethereum.State.lookupAccount,
                 Ethereum.State.updateAccount, Account.updateTransientStorage,
-                Stack.push, UInt256_ofNat_1, Sat256.natSub_zero, UInt256_subzero', hacc, hperm,
+                Stack.push, UInt256_ofNat_1, Sat256.subNat_zero, UInt256_subzero', hacc, hperm,
                 Option.option]
 
 theorem step_calldatacopy : ∀ (s : State),
@@ -2923,7 +2867,7 @@ theorem step_calldatacopy : ∀ (s : State),
         let memoryCost := memoryExpansionCost s .CALLDATACOPY
         if s.machineState.gasAvailable.toNat < memoryCost then .error .OutOfGass
         else
-        let gasAvailable' := s.machineState.gasAvailable.natSub memoryCost
+        let gasAvailable' := s.machineState.gasAvailable.subNat memoryCost
         let copyCost := GasConstants.Gverylow + GasConstants.Gcopy * ((c.toNat + 31) / 32)
         if gasAvailable'.toNat < copyCost then .error .OutOfGass
         else
@@ -2935,7 +2879,7 @@ theorem step_calldatacopy : ∀ (s : State),
                     s.executionEnv.calldata.write b.toNat s.machineState.memory a.toNat c.toNat
                   machineState.activeWords :=
                     UInt256.ofNat (MachineState.M s.machineState.activeWords.toNat a.toNat c.toNat)
-                  machineState.gasAvailable := gasAvailable'.natSub copyCost
+                  machineState.gasAvailable := gasAvailable'.subNat copyCost
                   machineState.pc := s.machineState.pc + ⟨1⟩
                   machineState.execLength := s.machineState.execLength + 1
                   }
@@ -2954,28 +2898,28 @@ theorem step_calldatacopy : ∀ (s : State),
       by_cases hmem : s.machineState.gasAvailable.toNat < memoryExpansionCost s .CALLDATACOPY
       · simp [hmem]
       · simp [hmem]
-        let gasAvailable' := s.machineState.gasAvailable.natSub (memoryExpansionCost s .CALLDATACOPY)
+        let gasAvailable' := s.machineState.gasAvailable.subNat (memoryExpansionCost s .CALLDATACOPY)
         let copyCost := GasConstants.Gverylow + GasConstants.Gcopy * ((c.toNat + 31) / 32)
         by_cases hgas : gasAvailable'.toNat < copyCost
         · have hgas' :
-              (s.machineState.gasAvailable.natSub
+              (s.machineState.gasAvailable.subNat
                     (Cₘ (UInt256.ofNat
                         (MachineState.M s.machineState.activeWords.toNat a.toNat c.toNat)) -
                         Cₘ s.machineState.activeWords)).toNat <
                 GasConstants.Gverylow + GasConstants.Gcopy * ((c.toNat + 31) / 32) := by
             simpa [gasAvailable', copyCost, memoryExpansionCost, memoryExpansionCost.μᵢ', hstack] using hgas
-          simp only [Sat256.natSub_toNat] at hgas'
+          simp only [Sat256.subNat_toNat] at hgas'
           simp [gasAvailable', copyCost, hgas', memoryExpansionCost, memoryExpansionCost.μᵢ', C', hstack,
             InstructionGasGroups.Wcopy]
         ·
           have hgas' :
-              ¬ (s.machineState.gasAvailable.natSub
+              ¬ (s.machineState.gasAvailable.subNat
                     (Cₘ (UInt256.ofNat
                         (MachineState.M s.machineState.activeWords.toNat a.toNat c.toNat)) -
                         Cₘ s.machineState.activeWords)).toNat <
                 GasConstants.Gverylow + GasConstants.Gcopy * ((c.toNat + 31) / 32) := by
             simpa [gasAvailable', copyCost, memoryExpansionCost, memoryExpansionCost.μᵢ', hstack] using hgas
-          simp only [Sat256.natSub_toNat] at hgas'
+          simp only [Sat256.subNat_toNat] at hgas'
           simp [gasAvailable', copyCost, hgas', memoryExpansionCost, memoryExpansionCost.μᵢ', C', hstack,
             InstructionGasGroups.Wcopy]
           simp [α, Operation.isCreate]
@@ -2998,7 +2942,7 @@ theorem step_codecopy : ∀ (s : State),
         let memoryCost := memoryExpansionCost s .CODECOPY
         if s.machineState.gasAvailable.toNat < memoryCost then .error .OutOfGass
         else
-        let gasAvailable' := s.machineState.gasAvailable.natSub memoryCost
+        let gasAvailable' := s.machineState.gasAvailable.subNat memoryCost
         let copyCost := GasConstants.Gverylow + GasConstants.Gcopy * ((c.toNat + 31) / 32)
         if gasAvailable'.toNat < copyCost then .error .OutOfGass
         else
@@ -3010,7 +2954,7 @@ theorem step_codecopy : ∀ (s : State),
                     s.executionEnv.code.write b.toNat s.machineState.memory a.toNat c.toNat
                   machineState.activeWords :=
                     UInt256.ofNat (MachineState.M s.machineState.activeWords.toNat a.toNat c.toNat)
-                  machineState.gasAvailable := gasAvailable'.natSub copyCost
+                  machineState.gasAvailable := gasAvailable'.subNat copyCost
                   machineState.pc := s.machineState.pc + ⟨1⟩
                   machineState.execLength := s.machineState.execLength + 1
                   }
@@ -3029,28 +2973,28 @@ theorem step_codecopy : ∀ (s : State),
       by_cases hmem : s.machineState.gasAvailable.toNat < memoryExpansionCost s .CODECOPY
       · simp [hmem]
       · simp [hmem]
-        let gasAvailable' := s.machineState.gasAvailable.natSub (memoryExpansionCost s .CODECOPY)
+        let gasAvailable' := s.machineState.gasAvailable.subNat (memoryExpansionCost s .CODECOPY)
         let copyCost := GasConstants.Gverylow + GasConstants.Gcopy * ((c.toNat + 31) / 32)
         by_cases hgas : gasAvailable'.toNat < copyCost
         · have hgas' :
-              (s.machineState.gasAvailable.natSub
+              (s.machineState.gasAvailable.subNat
                     (Cₘ (UInt256.ofNat
                         (MachineState.M s.machineState.activeWords.toNat a.toNat c.toNat)) -
                         Cₘ s.machineState.activeWords)).toNat <
                 GasConstants.Gverylow + GasConstants.Gcopy * ((c.toNat + 31) / 32) := by
             simpa [gasAvailable', copyCost, memoryExpansionCost, memoryExpansionCost.μᵢ', hstack] using hgas
-          simp only [Sat256.natSub_toNat] at hgas'
+          simp only [Sat256.subNat_toNat] at hgas'
           simp [gasAvailable', copyCost, hgas', memoryExpansionCost, memoryExpansionCost.μᵢ', C', hstack,
             InstructionGasGroups.Wcopy]
         ·
           have hgas' :
-              ¬ (s.machineState.gasAvailable.natSub
+              ¬ (s.machineState.gasAvailable.subNat
                     (Cₘ (UInt256.ofNat
                         (MachineState.M s.machineState.activeWords.toNat a.toNat c.toNat)) -
                         Cₘ s.machineState.activeWords)).toNat <
                 GasConstants.Gverylow + GasConstants.Gcopy * ((c.toNat + 31) / 32) := by
             simpa [gasAvailable', copyCost, memoryExpansionCost, memoryExpansionCost.μᵢ', hstack] using hgas
-          simp only [Sat256.natSub_toNat] at hgas'
+          simp only [Sat256.subNat_toNat] at hgas'
           simp [gasAvailable', copyCost, hgas', memoryExpansionCost, memoryExpansionCost.μᵢ', C', hstack,
             InstructionGasGroups.Wcopy]
           simp [α, Operation.isCreate]
@@ -3073,7 +3017,7 @@ theorem step_returndatacopy : ∀ (s : State),
         let memoryCost := memoryExpansionCost s .RETURNDATACOPY
         if s.machineState.gasAvailable.toNat < memoryCost then .error .OutOfGass
         else
-        let gasAvailable' := s.machineState.gasAvailable.natSub memoryCost
+        let gasAvailable' := s.machineState.gasAvailable.subNat memoryCost
         let copyCost := GasConstants.Gverylow + GasConstants.Gcopy * ((c.toNat + 31) / 32)
         if gasAvailable'.toNat < copyCost then .error .OutOfGass
         else if b.toNat + c.toNat > s.machineState.returnData.size then .error .InvalidMemoryAccess
@@ -3086,7 +3030,7 @@ theorem step_returndatacopy : ∀ (s : State),
                     s.machineState.returnData.write b.toNat s.machineState.memory a.toNat c.toNat
                   machineState.activeWords :=
                     UInt256.ofNat (MachineState.M s.machineState.activeWords.toNat a.toNat c.toNat)
-                  machineState.gasAvailable := gasAvailable'.natSub copyCost
+                  machineState.gasAvailable := gasAvailable'.subNat copyCost
                   machineState.pc := s.machineState.pc + ⟨1⟩
                   machineState.execLength := s.machineState.execLength + 1
                   }
@@ -3105,28 +3049,28 @@ theorem step_returndatacopy : ∀ (s : State),
       by_cases hmem : s.machineState.gasAvailable.toNat < memoryExpansionCost s .RETURNDATACOPY
       · simp [hmem]
       · simp [hmem]
-        let gasAvailable' := s.machineState.gasAvailable.natSub (memoryExpansionCost s .RETURNDATACOPY)
+        let gasAvailable' := s.machineState.gasAvailable.subNat (memoryExpansionCost s .RETURNDATACOPY)
         let copyCost := GasConstants.Gverylow + GasConstants.Gcopy * ((c.toNat + 31) / 32)
         by_cases hgas : gasAvailable'.toNat < copyCost
         · have hgas' :
-              (s.machineState.gasAvailable.natSub
+              (s.machineState.gasAvailable.subNat
                     (Cₘ (UInt256.ofNat
                         (MachineState.M s.machineState.activeWords.toNat a.toNat c.toNat)) -
                         Cₘ s.machineState.activeWords)).toNat <
                 GasConstants.Gverylow + GasConstants.Gcopy * ((c.toNat + 31) / 32) := by
             simpa [gasAvailable', copyCost, memoryExpansionCost, memoryExpansionCost.μᵢ', hstack] using hgas
-          simp only [Sat256.natSub_toNat] at hgas'
+          simp only [Sat256.subNat_toNat] at hgas'
           simp [gasAvailable', copyCost, hgas', memoryExpansionCost, memoryExpansionCost.μᵢ', C', hstack,
             InstructionGasGroups.Wcopy]
         ·
           have hgas' :
-              ¬ (s.machineState.gasAvailable.natSub
+              ¬ (s.machineState.gasAvailable.subNat
                     (Cₘ (UInt256.ofNat
                         (MachineState.M s.machineState.activeWords.toNat a.toNat c.toNat)) -
                         Cₘ s.machineState.activeWords)).toNat <
                 GasConstants.Gverylow + GasConstants.Gcopy * ((c.toNat + 31) / 32) := by
             simpa [gasAvailable', copyCost, memoryExpansionCost, memoryExpansionCost.μᵢ', hstack] using hgas
-          simp only [Sat256.natSub_toNat] at hgas'
+          simp only [Sat256.subNat_toNat] at hgas'
           simp [gasAvailable', copyCost, hgas', memoryExpansionCost, memoryExpansionCost.μᵢ', C', hstack,
             InstructionGasGroups.Wcopy]
           by_cases hreturn : b.toNat + c.toNat > s.machineState.returnData.size
@@ -3154,7 +3098,7 @@ theorem step_extcodecopy : ∀ (s : State),
         let memoryCost := memoryExpansionCost s .EXTCODECOPY
         if s.machineState.gasAvailable.toNat < memoryCost then .error .OutOfGass
         else
-        let gasAvailable' := s.machineState.gasAvailable.natSub memoryCost
+        let gasAvailable' := s.machineState.gasAvailable.subNat memoryCost
         let addr := AccountAddress.ofUInt256 a
         let copyCost := Caccess addr s.substate + GasConstants.Gcopy * ((d.toNat + 31) / 32)
         if gasAvailable'.toNat < copyCost then .error .OutOfGass
@@ -3168,7 +3112,7 @@ theorem step_extcodecopy : ∀ (s : State),
                   machineState.memory := code.write c.toNat s.machineState.memory b.toNat d.toNat
                   machineState.activeWords :=
                     UInt256.ofNat (MachineState.M s.machineState.activeWords.toNat b.toNat d.toNat)
-                  machineState.gasAvailable := gasAvailable'.natSub copyCost
+                  machineState.gasAvailable := gasAvailable'.subNat copyCost
                   machineState.pc := s.machineState.pc + ⟨1⟩
                   machineState.execLength := s.machineState.execLength + 1
                   }
@@ -3188,31 +3132,31 @@ theorem step_extcodecopy : ∀ (s : State),
       by_cases hmem : s.machineState.gasAvailable.toNat < memoryExpansionCost s .EXTCODECOPY
       · simp [hmem]
       · simp [hmem]
-        let gasAvailable' := s.machineState.gasAvailable.natSub (memoryExpansionCost s .EXTCODECOPY)
+        let gasAvailable' := s.machineState.gasAvailable.subNat (memoryExpansionCost s .EXTCODECOPY)
         let addr := AccountAddress.ofUInt256 a
         let copyCost := Caccess addr s.substate + GasConstants.Gcopy * ((d.toNat + 31) / 32)
         by_cases hgas : gasAvailable'.toNat < copyCost
         · have hgas' :
-              (s.machineState.gasAvailable.natSub
+              (s.machineState.gasAvailable.subNat
                     (Cₘ (UInt256.ofNat
                         (MachineState.M s.machineState.activeWords.toNat b.toNat d.toNat)) -
                         Cₘ s.machineState.activeWords)).toNat <
                 Caccess (AccountAddress.ofUInt256 a) s.substate +
                   GasConstants.Gcopy * ((d.toNat + 31) / 32) := by
             simpa [gasAvailable', addr, copyCost, memoryExpansionCost, memoryExpansionCost.μᵢ', hstack] using hgas
-          simp only [Sat256.natSub_toNat] at hgas'
+          simp only [Sat256.subNat_toNat] at hgas'
           simp [gasAvailable', addr, copyCost, hgas', memoryExpansionCost, memoryExpansionCost.μᵢ', C', hstack,
             InstructionGasGroups.Wcopy, InstructionGasGroups.Wextaccount]
         ·
           have hgas' :
-              ¬ (s.machineState.gasAvailable.natSub
+              ¬ (s.machineState.gasAvailable.subNat
                     (Cₘ (UInt256.ofNat
                         (MachineState.M s.machineState.activeWords.toNat b.toNat d.toNat)) -
                         Cₘ s.machineState.activeWords)).toNat <
                 Caccess (AccountAddress.ofUInt256 a) s.substate +
                   GasConstants.Gcopy * ((d.toNat + 31) / 32) := by
             simpa [gasAvailable', addr, copyCost, memoryExpansionCost, memoryExpansionCost.μᵢ', hstack] using hgas
-          simp only [Sat256.natSub_toNat] at hgas'
+          simp only [Sat256.subNat_toNat] at hgas'
           simp [gasAvailable', addr, copyCost, hgas', memoryExpansionCost, memoryExpansionCost.μᵢ', C', hstack,
             InstructionGasGroups.Wcopy, InstructionGasGroups.Wextaccount]
           simp [α, Operation.isCreate]
@@ -3236,7 +3180,7 @@ theorem step_mcopy : ∀ (s : State),
         let memoryCost := memoryExpansionCost s .MCOPY
         if s.machineState.gasAvailable.toNat < memoryCost then .error .OutOfGass
         else
-        let gasAvailable' := s.machineState.gasAvailable.natSub memoryCost
+        let gasAvailable' := s.machineState.gasAvailable.subNat memoryCost
         let copyCost := GasConstants.Gverylow + GasConstants.Gcopy * ((c.toNat + 31) / 32)
         if gasAvailable'.toNat < copyCost then .error .OutOfGass
         else
@@ -3248,7 +3192,7 @@ theorem step_mcopy : ∀ (s : State),
                   machineState.activeWords :=
                     UInt256.ofNat
                       (MachineState.M s.machineState.activeWords.toNat (max a.toNat b.toNat) c.toNat)
-                  machineState.gasAvailable := gasAvailable'.natSub copyCost
+                  machineState.gasAvailable := gasAvailable'.subNat copyCost
                   machineState.pc := s.machineState.pc + ⟨1⟩
                   machineState.execLength := s.machineState.execLength + 1
                   }
@@ -3267,28 +3211,28 @@ theorem step_mcopy : ∀ (s : State),
       by_cases hmem : s.machineState.gasAvailable.toNat < memoryExpansionCost s .MCOPY
       · simp [hmem]
       · simp [hmem]
-        let gasAvailable' := s.machineState.gasAvailable.natSub (memoryExpansionCost s .MCOPY)
+        let gasAvailable' := s.machineState.gasAvailable.subNat (memoryExpansionCost s .MCOPY)
         let copyCost := GasConstants.Gverylow + GasConstants.Gcopy * ((c.toNat + 31) / 32)
         by_cases hgas : gasAvailable'.toNat < copyCost
         · have hgas' :
-              (s.machineState.gasAvailable.natSub
+              (s.machineState.gasAvailable.subNat
                     (Cₘ (UInt256.ofNat
                         (MachineState.M s.machineState.activeWords.toNat (max a.toNat b.toNat) c.toNat)) -
                         Cₘ s.machineState.activeWords)).toNat <
                 GasConstants.Gverylow + GasConstants.Gcopy * ((c.toNat + 31) / 32) := by
             simpa [gasAvailable', copyCost, memoryExpansionCost, memoryExpansionCost.μᵢ', hstack] using hgas
-          simp only [Sat256.natSub_toNat] at hgas'
+          simp only [Sat256.subNat_toNat] at hgas'
           simp [gasAvailable', copyCost, hgas', memoryExpansionCost, memoryExpansionCost.μᵢ', C', hstack,
             InstructionGasGroups.Wcopy]
         ·
           have hgas' :
-              ¬ (s.machineState.gasAvailable.natSub
+              ¬ (s.machineState.gasAvailable.subNat
                     (Cₘ (UInt256.ofNat
                         (MachineState.M s.machineState.activeWords.toNat (max a.toNat b.toNat) c.toNat)) -
                         Cₘ s.machineState.activeWords)).toNat <
                 GasConstants.Gverylow + GasConstants.Gcopy * ((c.toNat + 31) / 32) := by
             simpa [gasAvailable', copyCost, memoryExpansionCost, memoryExpansionCost.μᵢ', hstack] using hgas
-          simp only [Sat256.natSub_toNat] at hgas'
+          simp only [Sat256.subNat_toNat] at hgas'
           simp [gasAvailable', copyCost, hgas', memoryExpansionCost, memoryExpansionCost.μᵢ', C', hstack,
             InstructionGasGroups.Wcopy]
           simp [α, Operation.isCreate]
@@ -3311,7 +3255,7 @@ theorem step_return : ∀ (s : State),
         let memoryCost := memoryExpansionCost s .RETURN
         if s.machineState.gasAvailable.toNat < memoryCost then .error .OutOfGass
         else
-        let gasAvailable' := s.machineState.gasAvailable.natSub memoryCost
+        let gasAvailable' := s.machineState.gasAvailable.subNat memoryCost
         if s.machineState.stack.length - 2 + 0 > 1024 then .error .StackOverflow
         else
         let output := s.machineState.memory.readWithPadding a.toNat b.toNat
@@ -3320,7 +3264,7 @@ theorem step_return : ∀ (s : State),
                   machineState.H_return := output
                   machineState.activeWords :=
                     UInt256.ofNat (MachineState.M s.machineState.activeWords.toNat a.toNat b.toNat)
-                  machineState.gasAvailable := gasAvailable'.natSub GasConstants.Gzero
+                  machineState.gasAvailable := gasAvailable'.subNat GasConstants.Gzero
                   machineState.pc := s.machineState.pc + ⟨1⟩
                   machineState.execLength := s.machineState.execLength + 1
                   }
@@ -3338,18 +3282,18 @@ theorem step_return : ∀ (s : State),
       by_cases hmem : s.machineState.gasAvailable.toNat < memoryExpansionCost s .RETURN
       · simp [hmem]
       · simp [hmem]
-        let gasAvailable' := s.machineState.gasAvailable.natSub (memoryExpansionCost s .RETURN)
+        let gasAvailable' := s.machineState.gasAvailable.subNat (memoryExpansionCost s .RETURN)
         by_cases hgas : gasAvailable'.toNat < GasConstants.Gzero
         · simp [GasConstants.Gzero] at hgas
         ·
           have hgas' :
-              ¬ (s.machineState.gasAvailable.natSub
+              ¬ (s.machineState.gasAvailable.subNat
                     (Cₘ (UInt256.ofNat
                         (MachineState.M s.machineState.activeWords.toNat a.toNat b.toNat)) -
                         Cₘ s.machineState.activeWords)).toNat <
                 GasConstants.Gzero := by
             simpa [gasAvailable', memoryExpansionCost, memoryExpansionCost.μᵢ', hstack] using hgas
-          simp only [Sat256.natSub_toNat] at hgas'
+          simp only [Sat256.subNat_toNat] at hgas'
           simp [gasAvailable', hgas', memoryExpansionCost, memoryExpansionCost.μᵢ', C', hstack,
             InstructionGasGroups.Wcopy, InstructionGasGroups.Wextaccount,
             InstructionGasGroups.Wzero]
@@ -3362,7 +3306,7 @@ theorem step_return : ∀ (s : State),
             unfold step
             simp [Id.run, EVM.binaryMachineStateOp, Stack.pop2, Ethereum.State.replaceStackAndIncrPC]
             unfold Ethereum.State.incrPC
-            simp [MachineState.evmReturn, UInt256_ofNat_1, Sat256.natSub_zero, UInt256_subzero']
+            simp [MachineState.evmReturn, UInt256_ofNat_1, Sat256.subNat_zero, UInt256_subzero']
 
 theorem step_revert : ∀ (s : State),
   let I_b := s.executionEnv.code
@@ -3373,7 +3317,7 @@ theorem step_revert : ∀ (s : State),
         let memoryCost := memoryExpansionCost s .REVERT
         if s.machineState.gasAvailable.toNat < memoryCost then .error .OutOfGass
         else
-        let gasAvailable' := s.machineState.gasAvailable.natSub memoryCost
+        let gasAvailable' := s.machineState.gasAvailable.subNat memoryCost
         if s.machineState.stack.length - 2 + 0 > 1024 then .error .StackOverflow
         else
         let output := s.machineState.memory.readWithPadding a.toNat b.toNat
@@ -3383,7 +3327,7 @@ theorem step_revert : ∀ (s : State),
                   machineState.activeWords :=
                     let m := MachineState.M s.machineState.activeWords.toNat a.toNat b.toNat
                     UInt256.ofNat (MachineState.M (UInt256.ofNat m).toNat a.toNat b.toNat)
-                  machineState.gasAvailable := gasAvailable'.natSub GasConstants.Gzero
+                  machineState.gasAvailable := gasAvailable'.subNat GasConstants.Gzero
                   machineState.pc := s.machineState.pc + ⟨1⟩
                   machineState.execLength := s.machineState.execLength + 1
                   }
@@ -3401,18 +3345,18 @@ theorem step_revert : ∀ (s : State),
       by_cases hmem : s.machineState.gasAvailable.toNat < memoryExpansionCost s .REVERT
       · simp [hmem]
       · simp [hmem]
-        let gasAvailable' := s.machineState.gasAvailable.natSub (memoryExpansionCost s .REVERT)
+        let gasAvailable' := s.machineState.gasAvailable.subNat (memoryExpansionCost s .REVERT)
         by_cases hgas : gasAvailable'.toNat < GasConstants.Gzero
         · simp [GasConstants.Gzero] at hgas
         ·
           have hgas' :
-              ¬ (s.machineState.gasAvailable.natSub
+              ¬ (s.machineState.gasAvailable.subNat
                     (Cₘ (UInt256.ofNat
                         (MachineState.M s.machineState.activeWords.toNat a.toNat b.toNat)) -
                         Cₘ s.machineState.activeWords)).toNat <
                 GasConstants.Gzero := by
             simpa [gasAvailable', memoryExpansionCost, memoryExpansionCost.μᵢ', hstack] using hgas
-          simp only [Sat256.natSub_toNat] at hgas'
+          simp only [Sat256.subNat_toNat] at hgas'
           simp [gasAvailable', hgas', memoryExpansionCost, memoryExpansionCost.μᵢ', C', hstack,
             InstructionGasGroups.Wcopy, InstructionGasGroups.Wextaccount,
             InstructionGasGroups.Wzero]
@@ -3425,7 +3369,7 @@ theorem step_revert : ∀ (s : State),
             unfold step
             simp [Id.run, EVM.binaryMachineStateOp, Stack.pop2, Ethereum.State.replaceStackAndIncrPC]
             unfold Ethereum.State.incrPC
-            simp [MachineState.evmRevert, MachineState.evmReturn, UInt256_ofNat_1, Sat256.natSub_zero, UInt256_subzero']
+            simp [MachineState.evmRevert, MachineState.evmReturn, UInt256_ofNat_1, Sat256.subNat_zero, UInt256_subzero']
 
 theorem step_log0 : ∀ (s : State),
   let I_b := s.executionEnv.code
@@ -3436,7 +3380,7 @@ theorem step_log0 : ∀ (s : State),
         let memoryCost := memoryExpansionCost s .LOG0
         if s.machineState.gasAvailable.toNat < memoryCost then .error .OutOfGass
         else
-        let gasAvailable' := s.machineState.gasAvailable.natSub memoryCost
+        let gasAvailable' := s.machineState.gasAvailable.subNat memoryCost
         let logCost := GasConstants.Glog + GasConstants.Glogdata * b.toNat
         if gasAvailable'.toNat < logCost then .error .OutOfGass
         else if s.machineState.stack.length - 2 + 0 > 1024 then .error .StackOverflow
@@ -3448,7 +3392,7 @@ theorem step_log0 : ∀ (s : State),
                   machineState.stack := t
                   machineState.activeWords :=
                     UInt256.ofNat (MachineState.M s.machineState.activeWords.toNat a.toNat b.toNat)
-                  machineState.gasAvailable := gasAvailable'.natSub logCost
+                  machineState.gasAvailable := gasAvailable'.subNat logCost
                   machineState.pc := s.machineState.pc + ⟨1⟩
                   machineState.execLength := s.machineState.execLength + 1
                   }
@@ -3466,27 +3410,27 @@ theorem step_log0 : ∀ (s : State),
       by_cases hmem : s.machineState.gasAvailable.toNat < memoryExpansionCost s .LOG0
       · simp [hmem]
       · simp [hmem]
-        let gasAvailable' := s.machineState.gasAvailable.natSub (memoryExpansionCost s .LOG0)
+        let gasAvailable' := s.machineState.gasAvailable.subNat (memoryExpansionCost s .LOG0)
         let logCost := GasConstants.Glog + GasConstants.Glogdata * b.toNat
         by_cases hgas : gasAvailable'.toNat < logCost
         · have hgas' :
-              (s.machineState.gasAvailable.natSub
+              (s.machineState.gasAvailable.subNat
                     (Cₘ (UInt256.ofNat
                         (MachineState.M s.machineState.activeWords.toNat a.toNat b.toNat)) -
                         Cₘ s.machineState.activeWords)).toNat <
                 GasConstants.Glog + GasConstants.Glogdata * b.toNat := by
             simpa [gasAvailable', logCost, memoryExpansionCost, memoryExpansionCost.μᵢ', hstack] using hgas
-          simp only [Sat256.natSub_toNat] at hgas'
+          simp only [Sat256.subNat_toNat] at hgas'
           simp [gasAvailable', logCost, hgas', memoryExpansionCost, memoryExpansionCost.μᵢ', C', hstack]
         ·
           have hgas' :
-              ¬ (s.machineState.gasAvailable.natSub
+              ¬ (s.machineState.gasAvailable.subNat
                     (Cₘ (UInt256.ofNat
                         (MachineState.M s.machineState.activeWords.toNat a.toNat b.toNat)) -
                         Cₘ s.machineState.activeWords)).toNat <
                 GasConstants.Glog + GasConstants.Glogdata * b.toNat := by
             simpa [gasAvailable', logCost, memoryExpansionCost, memoryExpansionCost.μᵢ', hstack] using hgas
-          simp only [Sat256.natSub_toNat] at hgas'
+          simp only [Sat256.subNat_toNat] at hgas'
           simp [gasAvailable', logCost, hgas', memoryExpansionCost, memoryExpansionCost.μᵢ', C', hstack]
           simp [α, Operation.isCreate]
           by_cases hoverflow : 1024 < t.length
@@ -3515,7 +3459,7 @@ theorem step_log1 : ∀ (s : State),
         let memoryCost := memoryExpansionCost s .LOG1
         if s.machineState.gasAvailable.toNat < memoryCost then .error .OutOfGass
         else
-        let gasAvailable' := s.machineState.gasAvailable.natSub memoryCost
+        let gasAvailable' := s.machineState.gasAvailable.subNat memoryCost
         let logCost := GasConstants.Glog + GasConstants.Glogdata * b.toNat + GasConstants.Glogtopic
         if gasAvailable'.toNat < logCost then .error .OutOfGass
         else if s.machineState.stack.length - 3 + 0 > 1024 then .error .StackOverflow
@@ -3527,7 +3471,7 @@ theorem step_log1 : ∀ (s : State),
                   machineState.stack := t
                   machineState.activeWords :=
                     UInt256.ofNat (MachineState.M s.machineState.activeWords.toNat a.toNat b.toNat)
-                  machineState.gasAvailable := gasAvailable'.natSub logCost
+                  machineState.gasAvailable := gasAvailable'.subNat logCost
                   machineState.pc := s.machineState.pc + ⟨1⟩
                   machineState.execLength := s.machineState.execLength + 1
                   }
@@ -3546,27 +3490,27 @@ theorem step_log1 : ∀ (s : State),
       by_cases hmem : s.machineState.gasAvailable.toNat < memoryExpansionCost s .LOG1
       · simp [hmem]
       · simp [hmem]
-        let gasAvailable' := s.machineState.gasAvailable.natSub (memoryExpansionCost s .LOG1)
+        let gasAvailable' := s.machineState.gasAvailable.subNat (memoryExpansionCost s .LOG1)
         let logCost := GasConstants.Glog + GasConstants.Glogdata * b.toNat + GasConstants.Glogtopic
         by_cases hgas : gasAvailable'.toNat < logCost
         · have hgas' :
-              (s.machineState.gasAvailable.natSub
+              (s.machineState.gasAvailable.subNat
                     (Cₘ (UInt256.ofNat
                         (MachineState.M s.machineState.activeWords.toNat a.toNat b.toNat)) -
                         Cₘ s.machineState.activeWords)).toNat <
                 GasConstants.Glog + GasConstants.Glogdata * b.toNat + GasConstants.Glogtopic := by
             simpa [gasAvailable', logCost, memoryExpansionCost, memoryExpansionCost.μᵢ', hstack] using hgas
-          simp only [Sat256.natSub_toNat] at hgas'
+          simp only [Sat256.subNat_toNat] at hgas'
           simp [gasAvailable', logCost, hgas', memoryExpansionCost, memoryExpansionCost.μᵢ', C', hstack]
         ·
           have hgas' :
-              ¬ (s.machineState.gasAvailable.natSub
+              ¬ (s.machineState.gasAvailable.subNat
                     (Cₘ (UInt256.ofNat
                         (MachineState.M s.machineState.activeWords.toNat a.toNat b.toNat)) -
                         Cₘ s.machineState.activeWords)).toNat <
                 GasConstants.Glog + GasConstants.Glogdata * b.toNat + GasConstants.Glogtopic := by
             simpa [gasAvailable', logCost, memoryExpansionCost, memoryExpansionCost.μᵢ', hstack] using hgas
-          simp only [Sat256.natSub_toNat] at hgas'
+          simp only [Sat256.subNat_toNat] at hgas'
           simp [gasAvailable', logCost, hgas', memoryExpansionCost, memoryExpansionCost.μᵢ', C', hstack]
           simp [α, Operation.isCreate]
           by_cases hoverflow : 1024 < t.length
@@ -3595,7 +3539,7 @@ theorem step_log2 : ∀ (s : State),
         let memoryCost := memoryExpansionCost s .LOG2
         if s.machineState.gasAvailable.toNat < memoryCost then .error .OutOfGass
         else
-        let gasAvailable' := s.machineState.gasAvailable.natSub memoryCost
+        let gasAvailable' := s.machineState.gasAvailable.subNat memoryCost
         let logCost := GasConstants.Glog + GasConstants.Glogdata * b.toNat + 2 * GasConstants.Glogtopic
         if gasAvailable'.toNat < logCost then .error .OutOfGass
         else if s.machineState.stack.length - 4 + 0 > 1024 then .error .StackOverflow
@@ -3607,7 +3551,7 @@ theorem step_log2 : ∀ (s : State),
                   machineState.stack := t
                   machineState.activeWords :=
                     UInt256.ofNat (MachineState.M s.machineState.activeWords.toNat a.toNat b.toNat)
-                  machineState.gasAvailable := gasAvailable'.natSub logCost
+                  machineState.gasAvailable := gasAvailable'.subNat logCost
                   machineState.pc := s.machineState.pc + ⟨1⟩
                   machineState.execLength := s.machineState.execLength + 1
                   }
@@ -3627,27 +3571,27 @@ theorem step_log2 : ∀ (s : State),
       by_cases hmem : s.machineState.gasAvailable.toNat < memoryExpansionCost s .LOG2
       · simp [hmem]
       · simp [hmem]
-        let gasAvailable' := s.machineState.gasAvailable.natSub (memoryExpansionCost s .LOG2)
+        let gasAvailable' := s.machineState.gasAvailable.subNat (memoryExpansionCost s .LOG2)
         let logCost := GasConstants.Glog + GasConstants.Glogdata * b.toNat + 2 * GasConstants.Glogtopic
         by_cases hgas : gasAvailable'.toNat < logCost
         · have hgas' :
-              (s.machineState.gasAvailable.natSub
+              (s.machineState.gasAvailable.subNat
                     (Cₘ (UInt256.ofNat
                         (MachineState.M s.machineState.activeWords.toNat a.toNat b.toNat)) -
                         Cₘ s.machineState.activeWords)).toNat <
                 GasConstants.Glog + GasConstants.Glogdata * b.toNat + 2 * GasConstants.Glogtopic := by
             simpa [gasAvailable', logCost, memoryExpansionCost, memoryExpansionCost.μᵢ', hstack] using hgas
-          simp only [Sat256.natSub_toNat] at hgas'
+          simp only [Sat256.subNat_toNat] at hgas'
           simp [gasAvailable', logCost, hgas', memoryExpansionCost, memoryExpansionCost.μᵢ', C', hstack]
         ·
           have hgas' :
-              ¬ (s.machineState.gasAvailable.natSub
+              ¬ (s.machineState.gasAvailable.subNat
                     (Cₘ (UInt256.ofNat
                         (MachineState.M s.machineState.activeWords.toNat a.toNat b.toNat)) -
                         Cₘ s.machineState.activeWords)).toNat <
                 GasConstants.Glog + GasConstants.Glogdata * b.toNat + 2 * GasConstants.Glogtopic := by
             simpa [gasAvailable', logCost, memoryExpansionCost, memoryExpansionCost.μᵢ', hstack] using hgas
-          simp only [Sat256.natSub_toNat] at hgas'
+          simp only [Sat256.subNat_toNat] at hgas'
           simp [gasAvailable', logCost, hgas', memoryExpansionCost, memoryExpansionCost.μᵢ', C', hstack]
           simp [α, Operation.isCreate]
           by_cases hoverflow : 1024 < t.length
@@ -3676,7 +3620,7 @@ theorem step_log3 : ∀ (s : State),
         let memoryCost := memoryExpansionCost s .LOG3
         if s.machineState.gasAvailable.toNat < memoryCost then .error .OutOfGass
         else
-        let gasAvailable' := s.machineState.gasAvailable.natSub memoryCost
+        let gasAvailable' := s.machineState.gasAvailable.subNat memoryCost
         let logCost := GasConstants.Glog + GasConstants.Glogdata * b.toNat + 3 * GasConstants.Glogtopic
         if gasAvailable'.toNat < logCost then .error .OutOfGass
         else if s.machineState.stack.length - 5 + 0 > 1024 then .error .StackOverflow
@@ -3688,7 +3632,7 @@ theorem step_log3 : ∀ (s : State),
                   machineState.stack := t
                   machineState.activeWords :=
                     UInt256.ofNat (MachineState.M s.machineState.activeWords.toNat a.toNat b.toNat)
-                  machineState.gasAvailable := gasAvailable'.natSub logCost
+                  machineState.gasAvailable := gasAvailable'.subNat logCost
                   machineState.pc := s.machineState.pc + ⟨1⟩
                   machineState.execLength := s.machineState.execLength + 1
                   }
@@ -3709,27 +3653,27 @@ theorem step_log3 : ∀ (s : State),
       by_cases hmem : s.machineState.gasAvailable.toNat < memoryExpansionCost s .LOG3
       · simp [hmem]
       · simp [hmem]
-        let gasAvailable' := s.machineState.gasAvailable.natSub (memoryExpansionCost s .LOG3)
+        let gasAvailable' := s.machineState.gasAvailable.subNat (memoryExpansionCost s .LOG3)
         let logCost := GasConstants.Glog + GasConstants.Glogdata * b.toNat + 3 * GasConstants.Glogtopic
         by_cases hgas : gasAvailable'.toNat < logCost
         · have hgas' :
-              (s.machineState.gasAvailable.natSub
+              (s.machineState.gasAvailable.subNat
                     (Cₘ (UInt256.ofNat
                         (MachineState.M s.machineState.activeWords.toNat a.toNat b.toNat)) -
                         Cₘ s.machineState.activeWords)).toNat <
                 GasConstants.Glog + GasConstants.Glogdata * b.toNat + 3 * GasConstants.Glogtopic := by
             simpa [gasAvailable', logCost, memoryExpansionCost, memoryExpansionCost.μᵢ', hstack] using hgas
-          simp only [Sat256.natSub_toNat] at hgas'
+          simp only [Sat256.subNat_toNat] at hgas'
           simp [gasAvailable', logCost, hgas', memoryExpansionCost, memoryExpansionCost.μᵢ', C', hstack]
         ·
           have hgas' :
-              ¬ (s.machineState.gasAvailable.natSub
+              ¬ (s.machineState.gasAvailable.subNat
                     (Cₘ (UInt256.ofNat
                         (MachineState.M s.machineState.activeWords.toNat a.toNat b.toNat)) -
                         Cₘ s.machineState.activeWords)).toNat <
                 GasConstants.Glog + GasConstants.Glogdata * b.toNat + 3 * GasConstants.Glogtopic := by
             simpa [gasAvailable', logCost, memoryExpansionCost, memoryExpansionCost.μᵢ', hstack] using hgas
-          simp only [Sat256.natSub_toNat] at hgas'
+          simp only [Sat256.subNat_toNat] at hgas'
           simp [gasAvailable', logCost, hgas', memoryExpansionCost, memoryExpansionCost.μᵢ', C', hstack]
           simp [α, Operation.isCreate]
           by_cases hoverflow : 1024 < t.length
@@ -3758,7 +3702,7 @@ theorem step_log4 : ∀ (s : State),
         let memoryCost := memoryExpansionCost s .LOG4
         if s.machineState.gasAvailable.toNat < memoryCost then .error .OutOfGass
         else
-        let gasAvailable' := s.machineState.gasAvailable.natSub memoryCost
+        let gasAvailable' := s.machineState.gasAvailable.subNat memoryCost
         let logCost := GasConstants.Glog + GasConstants.Glogdata * b.toNat + 4 * GasConstants.Glogtopic
         if gasAvailable'.toNat < logCost then .error .OutOfGass
         else if s.machineState.stack.length - 6 + 0 > 1024 then .error .StackOverflow
@@ -3770,7 +3714,7 @@ theorem step_log4 : ∀ (s : State),
                   machineState.stack := t
                   machineState.activeWords :=
                     UInt256.ofNat (MachineState.M s.machineState.activeWords.toNat a.toNat b.toNat)
-                  machineState.gasAvailable := gasAvailable'.natSub logCost
+                  machineState.gasAvailable := gasAvailable'.subNat logCost
                   machineState.pc := s.machineState.pc + ⟨1⟩
                   machineState.execLength := s.machineState.execLength + 1
                   }
@@ -3792,27 +3736,27 @@ theorem step_log4 : ∀ (s : State),
       by_cases hmem : s.machineState.gasAvailable.toNat < memoryExpansionCost s .LOG4
       · simp [hmem]
       · simp [hmem]
-        let gasAvailable' := s.machineState.gasAvailable.natSub (memoryExpansionCost s .LOG4)
+        let gasAvailable' := s.machineState.gasAvailable.subNat (memoryExpansionCost s .LOG4)
         let logCost := GasConstants.Glog + GasConstants.Glogdata * b.toNat + 4 * GasConstants.Glogtopic
         by_cases hgas : gasAvailable'.toNat < logCost
         · have hgas' :
-              (s.machineState.gasAvailable.natSub
+              (s.machineState.gasAvailable.subNat
                     (Cₘ (UInt256.ofNat
                         (MachineState.M s.machineState.activeWords.toNat a.toNat b.toNat)) -
                         Cₘ s.machineState.activeWords)).toNat <
                 GasConstants.Glog + GasConstants.Glogdata * b.toNat + 4 * GasConstants.Glogtopic := by
             simpa [gasAvailable', logCost, memoryExpansionCost, memoryExpansionCost.μᵢ', hstack] using hgas
-          simp only [Sat256.natSub_toNat] at hgas'
+          simp only [Sat256.subNat_toNat] at hgas'
           simp [gasAvailable', logCost, hgas', memoryExpansionCost, memoryExpansionCost.μᵢ', C', hstack]
         ·
           have hgas' :
-              ¬ (s.machineState.gasAvailable.natSub
+              ¬ (s.machineState.gasAvailable.subNat
                     (Cₘ (UInt256.ofNat
                         (MachineState.M s.machineState.activeWords.toNat a.toNat b.toNat)) -
                         Cₘ s.machineState.activeWords)).toNat <
                 GasConstants.Glog + GasConstants.Glogdata * b.toNat + 4 * GasConstants.Glogtopic := by
             simpa [gasAvailable', logCost, memoryExpansionCost, memoryExpansionCost.μᵢ', hstack] using hgas
-          simp only [Sat256.natSub_toNat] at hgas'
+          simp only [Sat256.subNat_toNat] at hgas'
           simp [gasAvailable', logCost, hgas', memoryExpansionCost, memoryExpansionCost.μᵢ', C', hstack]
           simp [α, Operation.isCreate]
           by_cases hoverflow : 1024 < t.length
@@ -3885,7 +3829,7 @@ theorem step_sstore : ∀ (s : State),
                   accountMap := accountMap
                   substate := substate
                   machineState.stack := t
-                  machineState.gasAvailable := s.machineState.gasAvailable.natSub gasCost
+                  machineState.gasAvailable := s.machineState.gasAvailable.subNat gasCost
                   machineState.pc := s.machineState.pc + ⟨1⟩
                   machineState.execLength := s.machineState.execLength + 1
                   }
@@ -3906,17 +3850,29 @@ theorem step_sstore : ∀ (s : State),
           machineState :=
             {s.machineState with
               stack := a :: b :: t
-              gasAvailable := s.machineState.gasAvailable.natSub 0}}
+              gasAvailable := s.machineState.gasAvailable.subNat 0}}
+      let prechargedState : State :=
+        {s with
+          machineState :=
+            {s.machineState with
+              stack := a :: b :: t}}
+      have hcostPre : Csstore prechargedState = Csstore s := by
+        simp [prechargedState, Csstore, hstack]
       by_cases hgas :
           (s.machineState.gasAvailable.toNat < Csstore chargedState)
       · simp [hgas, C', hstack, chargedState]
         have hgas0 : s.machineState.gasAvailable.toNat < Csstore s := by
-          simpa [chargedState, Csstore, hstack, Sat256.natSub_zero, UInt256_subzero'] using hgas
-        simp [hgas0]
+          simpa [chargedState, Csstore, hstack, Sat256.subNat_zero, UInt256_subzero'] using hgas
+        have hgasPre : s.machineState.gasAvailable.toNat < Csstore prechargedState := by
+          simpa [hcostPre] using hgas0
+        simp [prechargedState, hgasPre]
+        omega
       ·
         have hgas0 : ¬ s.machineState.gasAvailable.toNat < Csstore s := by
-          simpa [chargedState, Csstore, hstack, Sat256.natSub_zero, UInt256_subzero'] using hgas
-        simp [hgas, hgas0, C', hstack, chargedState]
+          simpa [chargedState, Csstore, hstack, Sat256.subNat_zero, UInt256_subzero'] using hgas
+        have hgasPre : ¬ s.machineState.gasAvailable.toNat < Csstore prechargedState := by
+          simpa [hcostPre] using hgas0
+        simp [hgas, hgas0, hgasPre, C', hstack, chargedState, prechargedState]
         simp [α, Operation.isCreate]
         by_cases hoverflow : 1024 < t.length
         · simp [hoverflow]
@@ -3931,15 +3887,15 @@ theorem step_sstore : ∀ (s : State),
               · rfl
             simp [hstatic, hperm]
             by_cases hstipend :
-                (s.machineState.gasAvailable.natSub 0).toNat ≤ GasConstants.Gcallstipend
+                (s.machineState.gasAvailable.subNat 0).toNat ≤ GasConstants.Gcallstipend
             · have hstipend0 :
                   s.machineState.gasAvailable.toNat ≤ GasConstants.Gcallstipend := by
-                simpa [Sat256.natSub_zero, UInt256_subzero'] using hstipend
+                simpa [Sat256.subNat_zero, UInt256_subzero'] using hstipend
               simp [hstipend, hstipend0]
             ·
               have hstipend0 :
                   ¬ s.machineState.gasAvailable.toNat ≤ GasConstants.Gcallstipend := by
-                simpa [Sat256.natSub_zero, UInt256_subzero'] using hstipend
+                simpa [Sat256.subNat_zero, UInt256_subzero'] using hstipend
               simp [hstipend, hstipend0, bind, Except.bind]
               unfold step
               simp [Id.run, binaryStateOp, Stack.pop2, Ethereum.State.replaceStackAndIncrPC]
@@ -3950,7 +3906,7 @@ theorem step_sstore : ∀ (s : State),
                 simp [Ethereum.State.sstore, Ethereum.State.lookupAccount,
                   Ethereum.State.setAccount, Ethereum.State.addAccessedStorageKey,
                   Ethereum.Substate.addAccessedStorageKey,
-                  Account.updateStorage, Stack.push, UInt256_ofNat_1, Sat256.natSub_zero, UInt256_subzero',
+                  Account.updateStorage, Stack.push, UInt256_ofNat_1, Sat256.subNat_zero, UInt256_subzero',
                   hacc, hperm, Option.option]
                 simp [Csstore, hstack, hgas0]
               | some acc =>
@@ -3960,7 +3916,7 @@ theorem step_sstore : ∀ (s : State),
                   simp [Ethereum.State.sstore, Ethereum.State.lookupAccount,
                     Ethereum.State.setAccount, Ethereum.State.addAccessedStorageKey,
                     Ethereum.Substate.addAccessedStorageKey,
-                    Account.updateStorage, Stack.push, UInt256_ofNat_1, Sat256.natSub_zero, UInt256_subzero',
+                    Account.updateStorage, Stack.push, UInt256_ofNat_1, Sat256.subNat_zero, UInt256_subzero',
                     hacc, hperm, Option.option]
                   rw [Account_fst_storage
                     (Batteries.RBMap.find! s.accountMap s.executionEnv.codeOwner)]
@@ -3982,7 +3938,7 @@ theorem step_call : ∀ (s : State),
         let memoryCost := memoryExpansionCost s .CALL
         if s.machineState.gasAvailable.toNat < memoryCost then .error .OutOfGass
         else
-          let gasAvailable' := s.machineState.gasAvailable.natSub memoryCost
+          let gasAvailable' := s.machineState.gasAvailable.subNat memoryCost
           let gasState := {s with machineState.gasAvailable := gasAvailable'}
           let gasCost :=
             Ccall (AccountAddress.ofUInt256 target) (AccountAddress.ofUInt256 target) value gas
@@ -4025,7 +3981,7 @@ theorem step_call : ∀ (s : State),
                   pc := s.machineState.pc + ⟨1⟩
                   memory := o.write 0 s.machineState.memory outOffset.toNat n.toNat
                   returnData := o
-                  gasAvailable := gasAvailable'.natSub (gasCost - g'.toNat)
+                  gasAvailable := gasAvailable'.subNat (gasCost - g'.toNat)
                   execLength := s.machineState.execLength + 1
                   activeWords :=
                     let m := MachineState.M s.machineState.activeWords.toNat inOffset.toNat inSize.toNat
@@ -4070,7 +4026,7 @@ theorem step_call : ∀ (s : State),
       by_cases hmem : s.machineState.gasAvailable.toNat < memoryExpansionCost s .CALL
       · simp [hmem, hnot_underflow]
       · simp [hmem]
-        let gasAvailable' := s.machineState.gasAvailable.natSub (memoryExpansionCost s .CALL)
+        let gasAvailable' := s.machineState.gasAvailable.subNat (memoryExpansionCost s .CALL)
         let gasState := {s with machineState.gasAvailable := gasAvailable'}
         let gasCost :=
           Ccall (AccountAddress.ofUInt256 target) (AccountAddress.ofUInt256 target) value gas
@@ -4089,11 +4045,11 @@ theorem step_call : ∀ (s : State),
                   { pc := s.machineState.pc,
                     stack := gas :: target :: value :: inOffset :: inSize :: outOffset :: outSize :: t,
                     execLength := s.machineState.execLength,
-                    gasAvailable := s.machineState.gasAvailable.natSub (memoryExpansionCost s .CALL),
+                    gasAvailable := s.machineState.gasAvailable.subNat (memoryExpansionCost s .CALL),
                     activeWords := s.machineState.activeWords, memory := s.machineState.memory,
                     returnData := s.machineState.returnData, H_return := s.machineState.H_return }
                   s.substate := by
-            simpa [gasAvailable', gasState, gasCost, hstk, Sat256.natSub_toNat] using hgas
+            simpa [gasAvailable', gasState, gasCost, hstk, Sat256.subNat_toNat] using hgas
           by_cases hoverflow : 1024 < t.length + 1
           · simp [gasAvailable', gasState, gasCost, hgas_not, C', hstk, α, hoverflow, hnot_underflow,
               Operation.isCreate]
@@ -4132,7 +4088,7 @@ theorem step_call' : ∀ (s : State),
         let memoryCost := memoryExpansionCost s .CALL
         if s.machineState.gasAvailable.toNat < memoryCost then .error .OutOfGass
         else
-          let gasAvailable' := s.machineState.gasAvailable.natSub memoryCost
+          let gasAvailable' := s.machineState.gasAvailable.subNat memoryCost
           let gasState := {s with machineState.gasAvailable := gasAvailable'}
           let gasCost :=
             Ccall (AccountAddress.ofUInt256 target) (AccountAddress.ofUInt256 target) value gas
@@ -4175,7 +4131,7 @@ theorem step_call' : ∀ (s : State),
                   pc := s.machineState.pc + ⟨1⟩
                   memory := o.write 0 s.machineState.memory outOffset.toNat n.toNat
                   returnData := o
-                  gasAvailable := gasAvailable'.natSub (gasCost - g'.toNat)
+                  gasAvailable := gasAvailable'.subNat (gasCost - g'.toNat)
                   execLength := s.machineState.execLength + 1
                   activeWords :=
                     let m := MachineState.M s.machineState.activeWords.toNat inOffset.toNat inSize.toNat
@@ -4195,7 +4151,7 @@ theorem step_callcode : ∀ (s : State),
         let memoryCost := memoryExpansionCost s .CALLCODE
         if s.machineState.gasAvailable.toNat < memoryCost then .error .OutOfGass
         else
-          let gasAvailable' := s.machineState.gasAvailable.natSub memoryCost
+          let gasAvailable' := s.machineState.gasAvailable.subNat memoryCost
           let gasState := {s with machineState.gasAvailable := gasAvailable'}
           let gasCost :=
             Ccall (AccountAddress.ofUInt256 target) s.executionEnv.codeOwner value gas
@@ -4237,7 +4193,7 @@ theorem step_callcode : ∀ (s : State),
                   pc := s.machineState.pc + ⟨1⟩
                   memory := o.write 0 s.machineState.memory outOffset.toNat n.toNat
                   returnData := o
-                  gasAvailable := gasAvailable'.natSub (gasCost - g'.toNat)
+                  gasAvailable := gasAvailable'.subNat (gasCost - g'.toNat)
                   execLength := s.machineState.execLength + 1
                   activeWords :=
                     let m := MachineState.M s.machineState.activeWords.toNat inOffset.toNat inSize.toNat
@@ -4282,7 +4238,7 @@ theorem step_callcode : ∀ (s : State),
       by_cases hmem : s.machineState.gasAvailable.toNat < memoryExpansionCost s .CALLCODE
       · simp [hmem, hnot_underflow]
       · simp [hmem]
-        let gasAvailable' := s.machineState.gasAvailable.natSub (memoryExpansionCost s .CALLCODE)
+        let gasAvailable' := s.machineState.gasAvailable.subNat (memoryExpansionCost s .CALLCODE)
         let gasState := {s with machineState.gasAvailable := gasAvailable'}
         let gasCost :=
           Ccall (AccountAddress.ofUInt256 target) s.executionEnv.codeOwner value gas
@@ -4301,11 +4257,11 @@ theorem step_callcode : ∀ (s : State),
                   { pc := s.machineState.pc,
                     stack := gas :: target :: value :: inOffset :: inSize :: outOffset :: outSize :: t,
                     execLength := s.machineState.execLength,
-                    gasAvailable := s.machineState.gasAvailable.natSub (memoryExpansionCost s .CALLCODE),
+                    gasAvailable := s.machineState.gasAvailable.subNat (memoryExpansionCost s .CALLCODE),
                     activeWords := s.machineState.activeWords, memory := s.machineState.memory,
                     returnData := s.machineState.returnData, H_return := s.machineState.H_return }
                   s.substate := by
-            simpa [gasAvailable', gasState, gasCost, hstk, Sat256.natSub_toNat] using hgas
+            simpa [gasAvailable', gasState, gasCost, hstk, Sat256.subNat_toNat] using hgas
           by_cases hoverflow : 1024 < t.length + 1
           · simp [gasAvailable', gasState, gasCost, hgas_not, C', hstk, α, hoverflow, hnot_underflow,
               Operation.isCreate]
@@ -4337,7 +4293,7 @@ theorem step_delegatecall : ∀ (s : State),
         let memoryCost := memoryExpansionCost s .DELEGATECALL
         if s.machineState.gasAvailable.toNat < memoryCost then .error .OutOfGass
         else
-          let gasAvailable' := s.machineState.gasAvailable.natSub memoryCost
+          let gasAvailable' := s.machineState.gasAvailable.subNat memoryCost
           let gasState := {s with machineState.gasAvailable := gasAvailable'}
           let value := (⟨0⟩ : UInt256)
           let gasCost :=
@@ -4381,7 +4337,7 @@ theorem step_delegatecall : ∀ (s : State),
                   pc := s.machineState.pc + ⟨1⟩
                   memory := o.write 0 s.machineState.memory outOffset.toNat n.toNat
                   returnData := o
-                  gasAvailable := gasAvailable'.natSub (gasCost - g'.toNat)
+                  gasAvailable := gasAvailable'.subNat (gasCost - g'.toNat)
                   execLength := s.machineState.execLength + 1
                   activeWords :=
                     let m := MachineState.M s.machineState.activeWords.toNat inOffset.toNat inSize.toNat
@@ -4422,7 +4378,7 @@ theorem step_delegatecall : ∀ (s : State),
       by_cases hmem : s.machineState.gasAvailable.toNat < memoryExpansionCost s .DELEGATECALL
       · simp [hmem, hnot_underflow]
       · simp [hmem]
-        let gasAvailable' := s.machineState.gasAvailable.natSub (memoryExpansionCost s .DELEGATECALL)
+        let gasAvailable' := s.machineState.gasAvailable.subNat (memoryExpansionCost s .DELEGATECALL)
         let gasState := {s with machineState.gasAvailable := gasAvailable'}
         let value := (⟨0⟩ : UInt256)
         let gasCost :=
@@ -4442,11 +4398,11 @@ theorem step_delegatecall : ∀ (s : State),
                   { pc := s.machineState.pc,
                     stack := gas :: target :: inOffset :: inSize :: outOffset :: outSize :: t,
                     execLength := s.machineState.execLength,
-                    gasAvailable := s.machineState.gasAvailable.natSub (memoryExpansionCost s .DELEGATECALL),
+                    gasAvailable := s.machineState.gasAvailable.subNat (memoryExpansionCost s .DELEGATECALL),
                     activeWords := s.machineState.activeWords, memory := s.machineState.memory,
                     returnData := s.machineState.returnData, H_return := s.machineState.H_return }
                   s.substate := by
-            simpa [gasAvailable', gasState, value, gasCost, hstk, Sat256.natSub_toNat] using hgas
+            simpa [gasAvailable', gasState, value, gasCost, hstk, Sat256.subNat_toNat] using hgas
           by_cases hoverflow : 1024 < t.length + 1
           · simp [gasAvailable', gasState, value, gasCost, hgas_not, C', hstk, α, hoverflow, hnot_underflow,
               Operation.isCreate]
@@ -4478,7 +4434,7 @@ theorem step_staticcall : ∀ (s : State),
         let memoryCost := memoryExpansionCost s .STATICCALL
         if s.machineState.gasAvailable.toNat < memoryCost then .error .OutOfGass
         else
-          let gasAvailable' := s.machineState.gasAvailable.natSub memoryCost
+          let gasAvailable' := s.machineState.gasAvailable.subNat memoryCost
           let gasState := {s with machineState.gasAvailable := gasAvailable'}
           let value := (⟨0⟩ : UInt256)
           let gasCost :=
@@ -4521,7 +4477,7 @@ theorem step_staticcall : ∀ (s : State),
                   pc := s.machineState.pc + ⟨1⟩
                   memory := o.write 0 s.machineState.memory outOffset.toNat n.toNat
                   returnData := o
-                  gasAvailable := gasAvailable'.natSub (gasCost - g'.toNat)
+                  gasAvailable := gasAvailable'.subNat (gasCost - g'.toNat)
                   execLength := s.machineState.execLength + 1
                   activeWords :=
                     let m := MachineState.M s.machineState.activeWords.toNat inOffset.toNat inSize.toNat
@@ -4562,7 +4518,7 @@ theorem step_staticcall : ∀ (s : State),
       by_cases hmem : s.machineState.gasAvailable.toNat < memoryExpansionCost s .STATICCALL
       · simp [hmem, hnot_underflow]
       · simp [hmem]
-        let gasAvailable' := s.machineState.gasAvailable.natSub (memoryExpansionCost s .STATICCALL)
+        let gasAvailable' := s.machineState.gasAvailable.subNat (memoryExpansionCost s .STATICCALL)
         let gasState := {s with machineState.gasAvailable := gasAvailable'}
         let value := (⟨0⟩ : UInt256)
         let gasCost :=
@@ -4582,11 +4538,11 @@ theorem step_staticcall : ∀ (s : State),
                   { pc := s.machineState.pc,
                     stack := gas :: target :: inOffset :: inSize :: outOffset :: outSize :: t,
                     execLength := s.machineState.execLength,
-                    gasAvailable := s.machineState.gasAvailable.natSub (memoryExpansionCost s .STATICCALL),
+                    gasAvailable := s.machineState.gasAvailable.subNat (memoryExpansionCost s .STATICCALL),
                     activeWords := s.machineState.activeWords, memory := s.machineState.memory,
                     returnData := s.machineState.returnData, H_return := s.machineState.H_return }
                   s.substate := by
-            simpa [gasAvailable', gasState, value, gasCost, hstk, Sat256.natSub_toNat] using hgas
+            simpa [gasAvailable', gasState, value, gasCost, hstk, Sat256.subNat_toNat] using hgas
           by_cases hoverflow : 1024 < t.length + 1
           · simp [gasAvailable', gasState, value, gasCost, hgas_not, C', hstk, α, hoverflow, hnot_underflow,
               Operation.isCreate]
@@ -4618,7 +4574,7 @@ theorem step_create : ∀ (s : State),
         let memoryCost := memoryExpansionCost s .CREATE
         if s.machineState.gasAvailable.toNat < memoryCost then .error .OutOfGass
         else
-        let gasAvailable' := s.machineState.gasAvailable.natSub memoryCost
+        let gasAvailable' := s.machineState.gasAvailable.subNat memoryCost
         let gasCost := GasConstants.Gcreate + R size.toNat
         if gasAvailable'.toNat < gasCost then .error .OutOfGass
         else if s.machineState.stack.length - 3 + 1 > 1024 then .error .StackOverflow
@@ -4627,7 +4583,7 @@ theorem step_create : ∀ (s : State),
         else
         let createState :=
           {s with
-            machineState.gasAvailable := gasAvailable'.natSub gasCost
+            machineState.gasAvailable := gasAvailable'.subNat gasCost
             machineState.execLength := s.machineState.execLength + 1}
         let initCode := createState.machineState.memory.readWithPadding offset.toNat size.toNat
         let Iₐ := createState.executionEnv.codeOwner
@@ -4663,7 +4619,7 @@ theorem step_create : ∀ (s : State),
                     UInt256.ofNat (MachineState.M createState.machineState.activeWords.toNat offset.toNat size.toNat)
                   machineState.returnData := newReturnData
                   machineState.gasAvailable :=
-                    createState.machineState.gasAvailable.natSub
+                    createState.machineState.gasAvailable.subNat
                       (L createState.machineState.gasAvailable.toNat - g'.toNat)
                   machineState.pc := createState.machineState.pc + ⟨1⟩
                   executionEnv := s.executionEnv
@@ -4698,33 +4654,33 @@ theorem step_create : ∀ (s : State),
               Cₘ (UInt256.ofNat (MachineState.M s.machineState.activeWords.toNat offset.toNat size.toNat)) -
                 Cₘ s.machineState.activeWords := by
           simpa [memoryExpansionCost, memoryExpansionCost.μᵢ', hstack] using hmem
-        let gasAvailable' := s.machineState.gasAvailable.natSub (memoryExpansionCost s .CREATE)
+        let gasAvailable' := s.machineState.gasAvailable.subNat (memoryExpansionCost s .CREATE)
         let gasCost := GasConstants.Gcreate + R size.toNat
         by_cases hgas : gasAvailable'.toNat < gasCost
         ·
-          have hgas' : (s.machineState.gasAvailable.natSub (memoryExpansionCost s .CREATE)).toNat <
+          have hgas' : (s.machineState.gasAvailable.subNat (memoryExpansionCost s .CREATE)).toNat <
               GasConstants.Gcreate + R size.toNat := by
             simpa [gasAvailable', gasCost] using hgas
           have hgas'' :
-              (s.machineState.gasAvailable.natSub
+              (s.machineState.gasAvailable.subNat
                     (Cₘ (UInt256.ofNat (MachineState.M s.machineState.activeWords.toNat offset.toNat size.toNat)) -
                         Cₘ s.machineState.activeWords)).toNat <
                 GasConstants.Gcreate + R size.toNat := by
             simpa [memoryExpansionCost, memoryExpansionCost.μᵢ', hstack] using hgas'
-          simp only [Sat256.natSub_toNat] at hgas''
+          simp only [Sat256.subNat_toNat] at hgas''
           simp [gasAvailable', gasCost, memoryExpansionCost, memoryExpansionCost.μᵢ',
             hmem', hgas', hgas'', C', hstack, hnot_underflow]
         ·
-          have hgas' : ¬ (s.machineState.gasAvailable.natSub (memoryExpansionCost s .CREATE)).toNat <
+          have hgas' : ¬ (s.machineState.gasAvailable.subNat (memoryExpansionCost s .CREATE)).toNat <
               GasConstants.Gcreate + R size.toNat := by
             simpa [gasAvailable', gasCost] using hgas
           have hgas'' :
-              ¬(s.machineState.gasAvailable.natSub
+              ¬(s.machineState.gasAvailable.subNat
                     (Cₘ (UInt256.ofNat (MachineState.M s.machineState.activeWords.toNat offset.toNat size.toNat)) -
                         Cₘ s.machineState.activeWords)).toNat <
                 GasConstants.Gcreate + R size.toNat := by
             simpa [memoryExpansionCost, memoryExpansionCost.μᵢ', hstack] using hgas'
-          simp only [Sat256.natSub_toNat] at hgas''
+          simp only [Sat256.subNat_toNat] at hgas''
           by_cases hoverflow : 1024 < t.length + 1
           ·
             have hoverflow' : s.machineState.stack.length - 3 + 1 > 1024 := by
@@ -4749,7 +4705,7 @@ theorem step_create : ∀ (s : State),
               ·
                 let createState : State :=
                   {s with
-                    machineState.gasAvailable := gasAvailable'.natSub gasCost
+                    machineState.gasAvailable := gasAvailable'.subNat gasCost
                     machineState.execLength := s.machineState.execLength + 1}
                 have hdepth_eq {hDepth : value ≤
                     (((createState.accountMap).find? createState.executionEnv.codeOwner).option ⟨0⟩ fun x => x.balance) ∧
@@ -4932,7 +4888,7 @@ theorem step_create2 : ∀ (s : State),
         let memoryCost := memoryExpansionCost s .CREATE2
         if s.machineState.gasAvailable.toNat < memoryCost then .error .OutOfGass
         else
-        let gasAvailable' := s.machineState.gasAvailable.natSub memoryCost
+        let gasAvailable' := s.machineState.gasAvailable.subNat memoryCost
         let gasCost := GasConstants.Gcreate + GasConstants.Gkeccak256word * ((size.toNat + 31) / 32) + R size.toNat
         if gasAvailable'.toNat < gasCost then .error .OutOfGass
         else if s.machineState.stack.length - 4 + 1 > 1024 then .error .StackOverflow
@@ -4941,7 +4897,7 @@ theorem step_create2 : ∀ (s : State),
         else
         let createState :=
           {s with
-            machineState.gasAvailable := gasAvailable'.natSub gasCost
+            machineState.gasAvailable := gasAvailable'.subNat gasCost
             machineState.execLength := s.machineState.execLength + 1}
         let initCode := createState.machineState.memory.readWithPadding offset.toNat size.toNat
         let ζ := Ethereum.UInt256.toByteArray salt
@@ -4978,7 +4934,7 @@ theorem step_create2 : ∀ (s : State),
                     UInt256.ofNat (MachineState.M createState.machineState.activeWords.toNat offset.toNat size.toNat)
                   machineState.returnData := newReturnData
                   machineState.gasAvailable :=
-                    createState.machineState.gasAvailable.natSub
+                    createState.machineState.gasAvailable.subNat
                       (L createState.machineState.gasAvailable.toNat - g'.toNat)
                   machineState.pc := createState.machineState.pc + ⟨1⟩
                   executionEnv := s.executionEnv
@@ -5015,33 +4971,33 @@ theorem step_create2 : ∀ (s : State),
               Cₘ (UInt256.ofNat (MachineState.M s.machineState.activeWords.toNat offset.toNat size.toNat)) -
                 Cₘ s.machineState.activeWords := by
           simpa [memoryExpansionCost, memoryExpansionCost.μᵢ', hstack] using hmem
-        let gasAvailable' := s.machineState.gasAvailable.natSub (memoryExpansionCost s .CREATE2)
+        let gasAvailable' := s.machineState.gasAvailable.subNat (memoryExpansionCost s .CREATE2)
         let gasCost := GasConstants.Gcreate + GasConstants.Gkeccak256word * ((size.toNat + 31) / 32) + R size.toNat
         by_cases hgas : gasAvailable'.toNat < gasCost
         ·
-          have hgas' : (s.machineState.gasAvailable.natSub (memoryExpansionCost s .CREATE2)).toNat <
+          have hgas' : (s.machineState.gasAvailable.subNat (memoryExpansionCost s .CREATE2)).toNat <
               GasConstants.Gcreate + GasConstants.Gkeccak256word * ((size.toNat + 31) / 32) + R size.toNat := by
             simpa [gasAvailable', gasCost] using hgas
           have hgas'' :
-              (s.machineState.gasAvailable.natSub
+              (s.machineState.gasAvailable.subNat
                     (Cₘ (UInt256.ofNat (MachineState.M s.machineState.activeWords.toNat offset.toNat size.toNat)) -
                         Cₘ s.machineState.activeWords)).toNat <
                 GasConstants.Gcreate + GasConstants.Gkeccak256word * ((size.toNat + 31) / 32) + R size.toNat := by
             simpa [memoryExpansionCost, memoryExpansionCost.μᵢ', hstack] using hgas'
-          simp only [Sat256.natSub_toNat] at hgas''
+          simp only [Sat256.subNat_toNat] at hgas''
           simp [gasAvailable', gasCost, memoryExpansionCost, memoryExpansionCost.μᵢ',
             hmem', hgas', hgas'', C', hstack, hnot_underflow]
         ·
-          have hgas' : ¬ (s.machineState.gasAvailable.natSub (memoryExpansionCost s .CREATE2)).toNat <
+          have hgas' : ¬ (s.machineState.gasAvailable.subNat (memoryExpansionCost s .CREATE2)).toNat <
               GasConstants.Gcreate + GasConstants.Gkeccak256word * ((size.toNat + 31) / 32) + R size.toNat := by
             simpa [gasAvailable', gasCost] using hgas
           have hgas'' :
-              ¬(s.machineState.gasAvailable.natSub
+              ¬(s.machineState.gasAvailable.subNat
                     (Cₘ (UInt256.ofNat (MachineState.M s.machineState.activeWords.toNat offset.toNat size.toNat)) -
                         Cₘ s.machineState.activeWords)).toNat <
                 GasConstants.Gcreate + GasConstants.Gkeccak256word * ((size.toNat + 31) / 32) + R size.toNat := by
             simpa [memoryExpansionCost, memoryExpansionCost.μᵢ', hstack] using hgas'
-          simp only [Sat256.natSub_toNat] at hgas''
+          simp only [Sat256.subNat_toNat] at hgas''
           by_cases hoverflow : 1024 < t.length + 1
           ·
             have hoverflow' : s.machineState.stack.length - 4 + 1 > 1024 := by
@@ -5066,7 +5022,7 @@ theorem step_create2 : ∀ (s : State),
               ·
                 let createState : State :=
                   {s with
-                    machineState.gasAvailable := gasAvailable'.natSub gasCost
+                    machineState.gasAvailable := gasAvailable'.subNat gasCost
                     machineState.execLength := s.machineState.execLength + 1}
                 have hdepth_eq {hDepth : value ≤
                     (((createState.accountMap).find? createState.executionEnv.codeOwner).option ⟨0⟩ fun x => x.balance) ∧
@@ -5254,7 +5210,7 @@ theorem step_selfdestruct : ∀ (s : State),
         else
         let sdState :=
           {s with
-            machineState.gasAvailable := s.machineState.gasAvailable.natSub gasCost
+            machineState.gasAvailable := s.machineState.gasAvailable.subNat gasCost
             machineState.execLength := s.machineState.execLength + 1}
         let Iₐ := sdState.executionEnv.codeOwner
         let r := AccountAddress.ofUInt256 target
@@ -5324,17 +5280,28 @@ theorem step_selfdestruct : ∀ (s : State),
             machineState :=
               {s.machineState with
                 stack := target :: t
-                gasAvailable := s.machineState.gasAvailable.natSub 0}}
+                gasAvailable := s.machineState.gasAvailable.subNat 0}}
+        let prechargedState : State :=
+          {s with
+            machineState :=
+              {s.machineState with
+                stack := target :: t}}
+        have hcostPre : Cselfdestruct prechargedState = Cselfdestruct s := by
+          simp [prechargedState, Cselfdestruct, hstack]
         by_cases hgas :
             (s.machineState.gasAvailable.toNat < Cselfdestruct chargedState)
         ·
           have hgas0 : s.machineState.gasAvailable.toNat < Cselfdestruct s := by
-            simpa [chargedState, Cselfdestruct, hstack, Sat256.natSub_zero, UInt256_subzero'] using hgas
-          simp [hgas, hgas0, C', hstack, chargedState]
+            simpa [chargedState, Cselfdestruct, hstack, Sat256.subNat_zero, UInt256_subzero'] using hgas
+          have hgasPre : s.machineState.gasAvailable.toNat < Cselfdestruct prechargedState := by
+            simpa [hcostPre] using hgas0
+          simp [hgas, hgas0, hgasPre, C', hstack, chargedState, prechargedState]
         ·
           have hgas0 : ¬ s.machineState.gasAvailable.toNat < Cselfdestruct s := by
-            simpa [chargedState, Cselfdestruct, hstack, Sat256.natSub_zero, UInt256_subzero'] using hgas
-          simp [hgas, hgas0, C', hstack, chargedState]
+            simpa [chargedState, Cselfdestruct, hstack, Sat256.subNat_zero, UInt256_subzero'] using hgas
+          have hgasPre : ¬ s.machineState.gasAvailable.toNat < Cselfdestruct prechargedState := by
+            simpa [hcostPre] using hgas0
+          simp [hgas, hgas0, hgasPre, C', hstack, chargedState, prechargedState]
           simp [α, Operation.isCreate]
           by_cases hoverflow : 1024 < t.length
           · simp [hoverflow]
@@ -5351,7 +5318,7 @@ theorem step_selfdestruct : ∀ (s : State),
               let gasCost := Cselfdestruct s
               let sdState :=
                 {s with
-                  machineState.gasAvailable := s.machineState.gasAvailable.natSub gasCost
+                  machineState.gasAvailable := s.machineState.gasAvailable.subNat gasCost
                   machineState.execLength := s.machineState.execLength + 1}
               let Iₐ := sdState.executionEnv.codeOwner
               let r := AccountAddress.ofUInt256 target
@@ -5367,7 +5334,7 @@ theorem step_selfdestruct : ∀ (s : State),
                     Batteries.RBMap.find? s.accountMap s.executionEnv.codeOwner with
                 | none =>
                   simp [hcreated, hcreated_mem, hself, dbgTrace, sdState, Iₐ, r, hgas0,
-                    chargedState, Cselfdestruct, hstack, Sat256.natSub_zero, UInt256_subzero', UInt256_ofNat_1]
+                    chargedState, Cselfdestruct, hstack, Sat256.subNat_zero, UInt256_subzero', UInt256_ofNat_1]
                 | some selfAcc =>
                   simp [hcreated, hcreated_mem, hself, sdState, Iₐ, r]
                   cases htarget :
@@ -5376,14 +5343,14 @@ theorem step_selfdestruct : ∀ (s : State),
                     simp [hcreated, hcreated_mem, htarget, sdState, Iₐ, r]
                     cases hbal : (selfAcc.balance == (⟨0⟩ : UInt256)) <;>
                       simp [hcreated, hcreated_mem, hbal, sdState, Iₐ, r, hgas0,
-                        chargedState, Cselfdestruct, hstack, Sat256.natSub_zero, UInt256_subzero', UInt256_ofNat_1]
+                        chargedState, Cselfdestruct, hstack, Sat256.subNat_zero, UInt256_subzero', UInt256_ofNat_1]
                   | some targetAcc =>
                     simp [hcreated, hcreated_mem, htarget, sdState, Iₐ, r]
                     by_cases hneq : AccountAddress.ofUInt256 target ≠ s.executionEnv.codeOwner
                     · simp [hcreated, hcreated_mem, hneq, sdState, Iₐ, r, hgas0,
-                        chargedState, Cselfdestruct, hstack, Sat256.natSub_zero, UInt256_subzero', UInt256_ofNat_1]
+                        chargedState, Cselfdestruct, hstack, Sat256.subNat_zero, UInt256_subzero', UInt256_ofNat_1]
                     · simp [hcreated, hcreated_mem, hneq, sdState, Iₐ, r, hgas0,
-                        chargedState, Cselfdestruct, hstack, Sat256.natSub_zero, UInt256_subzero', UInt256_ofNat_1]
+                        chargedState, Cselfdestruct, hstack, Sat256.subNat_zero, UInt256_subzero', UInt256_ofNat_1]
               · have hcreated_mem : s.executionEnv.codeOwner ∈ s.createdAccounts := by
                   rw [← Batteries.RBSet.contains_iff]
                   simp [hcreated]
@@ -5391,7 +5358,7 @@ theorem step_selfdestruct : ∀ (s : State),
                     Batteries.RBMap.find? s.accountMap s.executionEnv.codeOwner with
                 | none =>
                   simp [hcreated, hcreated_mem, hself, dbgTrace, sdState, Iₐ, r, hgas0,
-                    chargedState, Cselfdestruct, hstack, Sat256.natSub_zero, UInt256_subzero', UInt256_ofNat_1]
+                    chargedState, Cselfdestruct, hstack, Sat256.subNat_zero, UInt256_subzero', UInt256_ofNat_1]
                 | some selfAcc =>
                   simp [hcreated, hcreated_mem, hself, sdState, Iₐ, r]
                   cases htarget :
@@ -5400,14 +5367,14 @@ theorem step_selfdestruct : ∀ (s : State),
                     simp [hcreated, hcreated_mem, htarget, sdState, Iₐ, r]
                     cases hbal : (selfAcc.balance == (⟨0⟩ : UInt256)) <;>
                       simp [hcreated, hcreated_mem, hbal, sdState, Iₐ, r, hgas0,
-                        chargedState, Cselfdestruct, hstack, Sat256.natSub_zero, UInt256_subzero', UInt256_ofNat_1]
+                        chargedState, Cselfdestruct, hstack, Sat256.subNat_zero, UInt256_subzero', UInt256_ofNat_1]
                   | some targetAcc =>
                     simp [hcreated, hcreated_mem, htarget, sdState, Iₐ, r]
                     by_cases hneq : AccountAddress.ofUInt256 target ≠ s.executionEnv.codeOwner
                     · simp [hcreated, hcreated_mem, hneq, sdState, Iₐ, r, hgas0,
-                        chargedState, Cselfdestruct, hstack, Sat256.natSub_zero, UInt256_subzero', UInt256_ofNat_1]
+                        chargedState, Cselfdestruct, hstack, Sat256.subNat_zero, UInt256_subzero', UInt256_ofNat_1]
                     · simp [hcreated, hcreated_mem, hneq, sdState, Iₐ, r, hgas0,
-                        chargedState, Cselfdestruct, hstack, Sat256.natSub_zero, UInt256_subzero', UInt256_ofNat_1]
+                        chargedState, Cselfdestruct, hstack, Sat256.subNat_zero, UInt256_subzero', UInt256_ofNat_1]
 
 theorem step_pc : ∀ (s : State),
   let I_b := s.executionEnv.code
@@ -5419,7 +5386,7 @@ theorem step_pc : ∀ (s : State),
       else
       .ok ({s with
                 machineState.stack := s.machineState.pc :: s.machineState.stack,
-                machineState.gasAvailable := s.machineState.gasAvailable.natSub GasConstants.Gbase
+                machineState.gasAvailable := s.machineState.gasAvailable.subNat GasConstants.Gbase
                 machineState.pc := s.machineState.pc + ⟨1⟩
                 machineState.execLength := s.machineState.execLength + 1
                 }
@@ -5441,10 +5408,7 @@ theorem step_pc : ∀ (s : State),
         unfold step
         simp [Ethereum.State.replaceStackAndIncrPC]
         unfold Ethereum.State.incrPC
-        simp
-        apply And.intro
-        · simp [UInt256_ofNat_1]
-        · exact And.intro rfl rfl
+        simp [Stack.push, UInt256_ofNat_1]
 
 theorem step_msize : ∀ (s : State),
   let I_b := s.executionEnv.code
@@ -5456,7 +5420,7 @@ theorem step_msize : ∀ (s : State),
       else
       .ok ({s with
                 machineState.stack := (s.machineState.activeWords * ⟨32⟩) :: s.machineState.stack,
-                machineState.gasAvailable := s.machineState.gasAvailable.natSub GasConstants.Gbase
+                machineState.gasAvailable := s.machineState.gasAvailable.subNat GasConstants.Gbase
                 machineState.pc := s.machineState.pc + ⟨1⟩
                 machineState.execLength := s.machineState.execLength + 1
                 }
@@ -5478,11 +5442,7 @@ theorem step_msize : ∀ (s : State),
         unfold step
         simp [Id.run, EVM.machineStateOp, Ethereum.State.replaceStackAndIncrPC]
         unfold Ethereum.State.incrPC
-        simp
-        apply And.intro
-        · simp [UInt256_ofNat_1]
-        · simp [Stack.push, MachineState.msize]
-          rw [Sat256.natSub_zero]
+        simp [Stack.push, MachineState.msize, UInt256_ofNat_1]
 
 theorem step_gas : ∀ (s : State),
   let I_b := s.executionEnv.code
@@ -5494,8 +5454,8 @@ theorem step_gas : ∀ (s : State),
       else
       .ok ({s with
                 machineState.stack :=
-                  (s.machineState.gasAvailable.natSub GasConstants.Gbase).toUInt256 :: s.machineState.stack,
-                machineState.gasAvailable := s.machineState.gasAvailable.natSub GasConstants.Gbase
+                  (s.machineState.gasAvailable.subNat GasConstants.Gbase).toUInt256 :: s.machineState.stack,
+                machineState.gasAvailable := s.machineState.gasAvailable.subNat GasConstants.Gbase
                 machineState.pc := s.machineState.pc + ⟨1⟩
                 machineState.execLength := s.machineState.execLength + 1
                 }
@@ -5517,10 +5477,7 @@ theorem step_gas : ∀ (s : State),
         unfold step
         simp [Id.run, EVM.machineStateOp, Ethereum.State.replaceStackAndIncrPC, MachineState.gas]
         unfold Ethereum.State.incrPC
-        simp
-        apply And.intro
-        · simp [UInt256_ofNat_1]
-        · exact And.intro rfl rfl
+        simp [Stack.push, UInt256_ofNat_1]
 
 theorem step_jumpdest : ∀ (s : State),
   let I_b := s.executionEnv.code
@@ -5531,7 +5488,7 @@ theorem step_jumpdest : ∀ (s : State),
       if s.machineState.stack.length - 0 + 0 > 1024 then .error .StackOverflow
       else
       .ok ({s with
-                machineState.gasAvailable := s.machineState.gasAvailable.natSub GasConstants.Gjumpdest
+                machineState.gasAvailable := s.machineState.gasAvailable.subNat GasConstants.Gjumpdest
                 machineState.pc := s.machineState.pc + ⟨1⟩
                 machineState.execLength := s.machineState.execLength + 1
                 }
@@ -5550,10 +5507,7 @@ theorem step_jumpdest : ∀ (s : State),
         simp [bind, Except.bind]
         unfold step
         unfold Ethereum.State.incrPC
-        simp
-        apply And.intro
-        · simp [UInt256_ofNat_1]
-        · rw [Sat256.natSub_zero]
+        simp [UInt256_ofNat_1]
 
 theorem step_jump : ∀ (s : State),
   let I_b := s.executionEnv.code
@@ -5568,7 +5522,7 @@ theorem step_jump : ∀ (s : State),
         else
         .ok ({s with
                   machineState.stack := t,
-                  machineState.gasAvailable := s.machineState.gasAvailable.natSub GasConstants.Gmid
+                  machineState.gasAvailable := s.machineState.gasAvailable.subNat GasConstants.Gmid
                   machineState.pc := a
                   machineState.execLength := s.machineState.execLength + 1
                   }
@@ -5601,7 +5555,7 @@ theorem step_jump : ∀ (s : State),
             simp [I_b, hcontains, hoverflow]
             simp [bind, Except.bind]
             unfold step
-            simp [Stack.pop, Sat256.natSub_zero, UInt256_subzero']
+            simp [Stack.pop, Sat256.subNat_zero, UInt256_subzero']
 
 theorem step_jumpi : ∀ (s : State),
   let I_b := s.executionEnv.code
@@ -5616,7 +5570,7 @@ theorem step_jumpi : ∀ (s : State),
         else
         .ok ({s with
                   machineState.stack := t,
-                  machineState.gasAvailable := s.machineState.gasAvailable.natSub GasConstants.Ghigh
+                  machineState.gasAvailable := s.machineState.gasAvailable.subNat GasConstants.Ghigh
                   machineState.pc := if b != ⟨0⟩ then a else s.machineState.pc + ⟨1⟩
                   machineState.execLength := s.machineState.execLength + 1
                   }
@@ -5650,7 +5604,7 @@ theorem step_jumpi : ∀ (s : State),
             simp [I_b, hb, hbeq, hoverflow]
             simp [bind, Except.bind]
             unfold step
-            simp [Stack.pop2, hb, hbeq, hzero_bne, Sat256.natSub_zero, UInt256_subzero']
+            simp [Stack.pop2, hb, hbeq, hzero_bne, Sat256.subNat_zero, UInt256_subzero']
         ·
           have hbne : b ≠ (⟨0⟩ : UInt256) :=
             UInt256_bne_zero_eq_true_ne b hb
@@ -5668,7 +5622,7 @@ theorem step_jumpi : ∀ (s : State),
               simp [I_b, hb, hbne, hcontains, hoverflow]
               simp [bind, Except.bind]
               unfold step
-              simp [Stack.pop2, hb, hbne, Sat256.natSub_zero, UInt256_subzero']
+              simp [Stack.pop2, hb, hbne, Sat256.subNat_zero, UInt256_subzero']
 
 theorem step_push0 : ∀ (s : State),
   let I_b := s.executionEnv.code
@@ -5680,7 +5634,7 @@ theorem step_push0 : ∀ (s : State),
       else
       .ok ({s with
                 machineState.stack := ⟨0⟩ :: s.machineState.stack,
-                machineState.gasAvailable := s.machineState.gasAvailable.natSub GasConstants.Gbase
+                machineState.gasAvailable := s.machineState.gasAvailable.subNat GasConstants.Gbase
                 machineState.pc := s.machineState.pc + ⟨1⟩
                 machineState.execLength := s.machineState.execLength + 1
                 }
@@ -5702,11 +5656,7 @@ theorem step_push0 : ∀ (s : State),
         unfold step
         simp [Ethereum.State.replaceStackAndIncrPC]
         unfold Ethereum.State.incrPC
-        simp
-        apply And.intro
-        · simp [UInt256_ofNat_1]
-        · simp [Stack.push]
-          rw [Sat256.natSub_zero]
+        simp [Stack.push, UInt256_ofNat_1]
 
 set_option maxHeartbeats 2000000 in
 theorem step_push : ∀ (s : State) (op : Operation.POp) (arg : UInt256) (argWidth : Nat),
@@ -5720,7 +5670,7 @@ theorem step_push : ∀ (s : State) (op : Operation.POp) (arg : UInt256) (argWid
       else
       .ok ({s with
                 machineState.stack := arg :: s.machineState.stack,
-                machineState.gasAvailable := s.machineState.gasAvailable.natSub GasConstants.Gverylow
+                machineState.gasAvailable := s.machineState.gasAvailable.subNat GasConstants.Gverylow
                 machineState.pc := s.machineState.pc + UInt256.ofNat argWidth.succ
                 machineState.execLength := s.machineState.execLength + 1
                 }
@@ -5731,7 +5681,7 @@ theorem step_push : ∀ (s : State) (op : Operation.POp) (arg : UInt256) (argWid
       {s with
         machineState :=
           {s.machineState with
-            gasAvailable := s.machineState.gasAvailable.natSub 0}}
+            gasAvailable := s.machineState.gasAvailable.subNat 0}}
     have hcostCharged : C' chargedState (.Push op) = GasConstants.Gverylow := by
       cases op
       · contradiction
@@ -5740,12 +5690,20 @@ theorem step_push : ∀ (s : State) (op : Operation.POp) (arg : UInt256) (argWid
           InstructionGasGroups.Wzero, InstructionGasGroups.Wbase,
           InstructionGasGroups.Wverylow, InstructionGasGroups.Wverylow.pushInstrsWithoutZero,
           InstructionGasGroups.Wverylow.dupInstrs, InstructionGasGroups.Wverylow.swapInstrs]
+    have hcost : C' s (.Push op) = GasConstants.Gverylow := by
+      cases op
+      · contradiction
+      all_goals
+        simp [C', InstructionGasGroups.Wcopy, InstructionGasGroups.Wextaccount,
+          InstructionGasGroups.Wzero, InstructionGasGroups.Wbase,
+          InstructionGasGroups.Wverylow, InstructionGasGroups.Wverylow.pushInstrsWithoutZero,
+          InstructionGasGroups.Wverylow.dupInstrs, InstructionGasGroups.Wverylow.swapInstrs]
     simp [Xstep, Z, δ, I_b, hpush]
-    simp [memoryExpansionCost, memoryExpansionCost.μᵢ', hcostCharged]
+    simp [memoryExpansionCost, memoryExpansionCost.μᵢ', hcostCharged, hcost]
     by_cases hgas :
       (s.machineState.gasAvailable.toNat < GasConstants.Gverylow)
-    · simp [hgas, hcostCharged, chargedState]
-    · simp [hgas, hcostCharged, chargedState, α, Operation.isCreate]
+    · simp [hgas, hcostCharged, hcost, chargedState]
+    · simp [hgas, hcostCharged, hcost, chargedState, α, Operation.isCreate]
       by_cases hoverflow : 1024 < s.machineState.stack.length + 1
       · simp [hoverflow]
       ·
@@ -5755,7 +5713,7 @@ theorem step_push : ∀ (s : State) (op : Operation.POp) (arg : UInt256) (argWid
         · contradiction
         all_goals
           simp [Ethereum.State.replaceStackAndIncrPC, Ethereum.State.incrPC,
-            Stack.push, Sat256.natSub_zero, UInt256_subzero', Id.run]
+            Stack.push, Sat256.subNat_zero, UInt256_subzero', Id.run]
 
 theorem step_push1 : ∀ (s : State) (arg : UInt256),
   let I_b := s.executionEnv.code
@@ -5765,7 +5723,7 @@ theorem step_push1 : ∀ (s : State) (arg : UInt256),
       else if s.machineState.stack.length - 0 + 1 > 1024 then .error .StackOverflow
       else .ok ({s with
         machineState.stack := arg :: s.machineState.stack
-        machineState.gasAvailable := s.machineState.gasAvailable.natSub GasConstants.Gverylow
+        machineState.gasAvailable := s.machineState.gasAvailable.subNat GasConstants.Gverylow
         machineState.pc := s.machineState.pc + UInt256.ofNat 2
         machineState.execLength := s.machineState.execLength + 1}, .none)
 := by
@@ -5780,7 +5738,7 @@ theorem step_push2 : ∀ (s : State) (arg : UInt256),
       else if s.machineState.stack.length - 0 + 1 > 1024 then .error .StackOverflow
       else .ok ({s with
         machineState.stack := arg :: s.machineState.stack
-        machineState.gasAvailable := s.machineState.gasAvailable.natSub GasConstants.Gverylow
+        machineState.gasAvailable := s.machineState.gasAvailable.subNat GasConstants.Gverylow
         machineState.pc := s.machineState.pc + UInt256.ofNat 3
         machineState.execLength := s.machineState.execLength + 1}, .none)
 := by
@@ -5795,7 +5753,7 @@ theorem step_push3 : ∀ (s : State) (arg : UInt256),
       else if s.machineState.stack.length - 0 + 1 > 1024 then .error .StackOverflow
       else .ok ({s with
         machineState.stack := arg :: s.machineState.stack
-        machineState.gasAvailable := s.machineState.gasAvailable.natSub GasConstants.Gverylow
+        machineState.gasAvailable := s.machineState.gasAvailable.subNat GasConstants.Gverylow
         machineState.pc := s.machineState.pc + UInt256.ofNat 4
         machineState.execLength := s.machineState.execLength + 1}, .none)
 := by
@@ -5810,7 +5768,7 @@ theorem step_push4 : ∀ (s : State) (arg : UInt256),
       else if s.machineState.stack.length - 0 + 1 > 1024 then .error .StackOverflow
       else .ok ({s with
         machineState.stack := arg :: s.machineState.stack
-        machineState.gasAvailable := s.machineState.gasAvailable.natSub GasConstants.Gverylow
+        machineState.gasAvailable := s.machineState.gasAvailable.subNat GasConstants.Gverylow
         machineState.pc := s.machineState.pc + UInt256.ofNat 5
         machineState.execLength := s.machineState.execLength + 1}, .none)
 := by
@@ -5825,7 +5783,7 @@ theorem step_push5 : ∀ (s : State) (arg : UInt256),
       else if s.machineState.stack.length - 0 + 1 > 1024 then .error .StackOverflow
       else .ok ({s with
         machineState.stack := arg :: s.machineState.stack
-        machineState.gasAvailable := s.machineState.gasAvailable.natSub GasConstants.Gverylow
+        machineState.gasAvailable := s.machineState.gasAvailable.subNat GasConstants.Gverylow
         machineState.pc := s.machineState.pc + UInt256.ofNat 6
         machineState.execLength := s.machineState.execLength + 1}, .none)
 := by
@@ -5840,7 +5798,7 @@ theorem step_push6 : ∀ (s : State) (arg : UInt256),
       else if s.machineState.stack.length - 0 + 1 > 1024 then .error .StackOverflow
       else .ok ({s with
         machineState.stack := arg :: s.machineState.stack
-        machineState.gasAvailable := s.machineState.gasAvailable.natSub GasConstants.Gverylow
+        machineState.gasAvailable := s.machineState.gasAvailable.subNat GasConstants.Gverylow
         machineState.pc := s.machineState.pc + UInt256.ofNat 7
         machineState.execLength := s.machineState.execLength + 1}, .none)
 := by
@@ -5855,7 +5813,7 @@ theorem step_push7 : ∀ (s : State) (arg : UInt256),
       else if s.machineState.stack.length - 0 + 1 > 1024 then .error .StackOverflow
       else .ok ({s with
         machineState.stack := arg :: s.machineState.stack
-        machineState.gasAvailable := s.machineState.gasAvailable.natSub GasConstants.Gverylow
+        machineState.gasAvailable := s.machineState.gasAvailable.subNat GasConstants.Gverylow
         machineState.pc := s.machineState.pc + UInt256.ofNat 8
         machineState.execLength := s.machineState.execLength + 1}, .none)
 := by
@@ -5870,7 +5828,7 @@ theorem step_push8 : ∀ (s : State) (arg : UInt256),
       else if s.machineState.stack.length - 0 + 1 > 1024 then .error .StackOverflow
       else .ok ({s with
         machineState.stack := arg :: s.machineState.stack
-        machineState.gasAvailable := s.machineState.gasAvailable.natSub GasConstants.Gverylow
+        machineState.gasAvailable := s.machineState.gasAvailable.subNat GasConstants.Gverylow
         machineState.pc := s.machineState.pc + UInt256.ofNat 9
         machineState.execLength := s.machineState.execLength + 1}, .none)
 := by
@@ -5885,7 +5843,7 @@ theorem step_push9 : ∀ (s : State) (arg : UInt256),
       else if s.machineState.stack.length - 0 + 1 > 1024 then .error .StackOverflow
       else .ok ({s with
         machineState.stack := arg :: s.machineState.stack
-        machineState.gasAvailable := s.machineState.gasAvailable.natSub GasConstants.Gverylow
+        machineState.gasAvailable := s.machineState.gasAvailable.subNat GasConstants.Gverylow
         machineState.pc := s.machineState.pc + UInt256.ofNat 10
         machineState.execLength := s.machineState.execLength + 1}, .none)
 := by
@@ -5900,7 +5858,7 @@ theorem step_push10 : ∀ (s : State) (arg : UInt256),
       else if s.machineState.stack.length - 0 + 1 > 1024 then .error .StackOverflow
       else .ok ({s with
         machineState.stack := arg :: s.machineState.stack
-        machineState.gasAvailable := s.machineState.gasAvailable.natSub GasConstants.Gverylow
+        machineState.gasAvailable := s.machineState.gasAvailable.subNat GasConstants.Gverylow
         machineState.pc := s.machineState.pc + UInt256.ofNat 11
         machineState.execLength := s.machineState.execLength + 1}, .none)
 := by
@@ -5918,7 +5876,7 @@ theorem step_dup1 : ∀ (s : State),
         else
         .ok ({s with
                   machineState.stack := a :: a :: t,
-                  machineState.gasAvailable := s.machineState.gasAvailable.natSub GasConstants.Gverylow
+                  machineState.gasAvailable := s.machineState.gasAvailable.subNat GasConstants.Gverylow
                   machineState.pc := s.machineState.pc + ⟨1⟩
                   machineState.execLength := s.machineState.execLength + 1
                   }
@@ -5950,10 +5908,7 @@ theorem step_dup1 : ∀ (s : State),
           unfold step
           simp [EVM.dup, Ethereum.State.replaceStackAndIncrPC]
           unfold Ethereum.State.incrPC
-          simp
-          apply And.intro
-          · simp [UInt256_ofNat_1]
-          · rw [Sat256.natSub_zero]
+          simp [UInt256_ofNat_1, Sat256.subNat_zero]
 
 theorem step_dup2 : ∀ (s : State),
   let I_b := s.executionEnv.code
@@ -5967,7 +5922,7 @@ theorem step_dup2 : ∀ (s : State),
         else
         .ok ({s with
                   machineState.stack := b :: a :: b :: t,
-                  machineState.gasAvailable := s.machineState.gasAvailable.natSub GasConstants.Gverylow
+                  machineState.gasAvailable := s.machineState.gasAvailable.subNat GasConstants.Gverylow
                   machineState.pc := s.machineState.pc + ⟨1⟩
                   machineState.execLength := s.machineState.execLength + 1
                   }
@@ -6000,10 +5955,7 @@ theorem step_dup2 : ∀ (s : State),
           unfold step
           simp [EVM.dup, Ethereum.State.replaceStackAndIncrPC]
           unfold Ethereum.State.incrPC
-          simp
-          apply And.intro
-          · simp [UInt256_ofNat_1]
-          · rw [Sat256.natSub_zero]
+          simp [UInt256_ofNat_1, Sat256.subNat_zero]
 
 theorem step_swap1 : ∀ (s : State),
   let I_b := s.executionEnv.code
@@ -6017,7 +5969,7 @@ theorem step_swap1 : ∀ (s : State),
         else
         .ok ({s with
                   machineState.stack := b :: a :: t,
-                  machineState.gasAvailable := s.machineState.gasAvailable.natSub GasConstants.Gverylow
+                  machineState.gasAvailable := s.machineState.gasAvailable.subNat GasConstants.Gverylow
                   machineState.pc := s.machineState.pc + ⟨1⟩
                   machineState.execLength := s.machineState.execLength + 1
                   }
@@ -6050,10 +6002,7 @@ theorem step_swap1 : ∀ (s : State),
           unfold step
           simp [EVM.swap, Ethereum.State.replaceStackAndIncrPC]
           unfold Ethereum.State.incrPC
-          simp
-          apply And.intro
-          · simp [UInt256_ofNat_1]
-          · rw [Sat256.natSub_zero]
+          simp [UInt256_ofNat_1, Sat256.subNat_zero]
 theorem step_swap2 : ∀ (s : State),
   let I_b := s.executionEnv.code
   decode I_b s.machineState.pc = some (.SWAP2, .none)
@@ -6066,7 +6015,7 @@ theorem step_swap2 : ∀ (s : State),
         else
         .ok ({s with
                   machineState.stack := c :: b :: a :: t,
-                  machineState.gasAvailable := s.machineState.gasAvailable.natSub GasConstants.Gverylow
+                  machineState.gasAvailable := s.machineState.gasAvailable.subNat GasConstants.Gverylow
                   machineState.pc := s.machineState.pc + ⟨1⟩
                   machineState.execLength := s.machineState.execLength + 1
                   }
@@ -6100,10 +6049,7 @@ theorem step_swap2 : ∀ (s : State),
           unfold step
           simp [EVM.swap, Ethereum.State.replaceStackAndIncrPC]
           unfold Ethereum.State.incrPC
-          simp
-          apply And.intro
-          · simp [UInt256_ofNat_1]
-          · rw [Sat256.natSub_zero]
+          simp [UInt256_ofNat_1, Sat256.subNat_zero]
 
 theorem step_dup3 : ∀ (s : State),
   let I_b := s.executionEnv.code
@@ -6117,7 +6063,7 @@ theorem step_dup3 : ∀ (s : State),
         else
         .ok ({s with
                   machineState.stack := c :: a :: b :: c :: t,
-                  machineState.gasAvailable := s.machineState.gasAvailable.natSub GasConstants.Gverylow
+                  machineState.gasAvailable := s.machineState.gasAvailable.subNat GasConstants.Gverylow
                   machineState.pc := s.machineState.pc + ⟨1⟩
                   machineState.execLength := s.machineState.execLength + 1
                   }
@@ -6151,10 +6097,7 @@ theorem step_dup3 : ∀ (s : State),
           unfold step
           simp [EVM.dup, Ethereum.State.replaceStackAndIncrPC]
           unfold Ethereum.State.incrPC
-          simp
-          apply And.intro
-          · simp [UInt256_ofNat_1]
-          · rw [Sat256.natSub_zero]
+          simp [UInt256_ofNat_1, Sat256.subNat_zero]
 
 theorem step_swap3 : ∀ (s : State),
   let I_b := s.executionEnv.code
@@ -6168,7 +6111,7 @@ theorem step_swap3 : ∀ (s : State),
         else
         .ok ({s with
                   machineState.stack := d :: b :: c :: a :: t,
-                  machineState.gasAvailable := s.machineState.gasAvailable.natSub GasConstants.Gverylow
+                  machineState.gasAvailable := s.machineState.gasAvailable.subNat GasConstants.Gverylow
                   machineState.pc := s.machineState.pc + ⟨1⟩
                   machineState.execLength := s.machineState.execLength + 1
                   }
@@ -6203,10 +6146,7 @@ theorem step_swap3 : ∀ (s : State),
           unfold step
           simp [EVM.swap, Ethereum.State.replaceStackAndIncrPC]
           unfold Ethereum.State.incrPC
-          simp
-          apply And.intro
-          · simp [UInt256_ofNat_1]
-          · rw [Sat256.natSub_zero]
+          simp [UInt256_ofNat_1, Sat256.subNat_zero]
 
 theorem step_dup4 : ∀ (s : State),
   let I_b := s.executionEnv.code
@@ -6220,7 +6160,7 @@ theorem step_dup4 : ∀ (s : State),
         else
         .ok ({s with
                   machineState.stack := d :: a :: b :: c :: d :: t,
-                  machineState.gasAvailable := s.machineState.gasAvailable.natSub GasConstants.Gverylow
+                  machineState.gasAvailable := s.machineState.gasAvailable.subNat GasConstants.Gverylow
                   machineState.pc := s.machineState.pc + ⟨1⟩
                   machineState.execLength := s.machineState.execLength + 1
                   }
@@ -6255,10 +6195,7 @@ theorem step_dup4 : ∀ (s : State),
           unfold step
           simp [EVM.dup, Ethereum.State.replaceStackAndIncrPC]
           unfold Ethereum.State.incrPC
-          simp
-          apply And.intro
-          · simp [UInt256_ofNat_1]
-          · rw [Sat256.natSub_zero]
+          simp [UInt256_ofNat_1, Sat256.subNat_zero]
 
 theorem step_swap4 : ∀ (s : State),
   let I_b := s.executionEnv.code
@@ -6272,7 +6209,7 @@ theorem step_swap4 : ∀ (s : State),
         else
         .ok ({s with
                   machineState.stack := e :: b :: c :: d :: a :: t,
-                  machineState.gasAvailable := s.machineState.gasAvailable.natSub GasConstants.Gverylow
+                  machineState.gasAvailable := s.machineState.gasAvailable.subNat GasConstants.Gverylow
                   machineState.pc := s.machineState.pc + ⟨1⟩
                   machineState.execLength := s.machineState.execLength + 1
                   }
@@ -6308,10 +6245,7 @@ theorem step_swap4 : ∀ (s : State),
           unfold step
           simp [EVM.swap, Ethereum.State.replaceStackAndIncrPC]
           unfold Ethereum.State.incrPC
-          simp
-          apply And.intro
-          · simp [UInt256_ofNat_1]
-          · rw [Sat256.natSub_zero]
+          simp [UInt256_ofNat_1, Sat256.subNat_zero]
 
 theorem step_dup5 : ∀ (s : State),
   let I_b := s.executionEnv.code
@@ -6325,7 +6259,7 @@ theorem step_dup5 : ∀ (s : State),
         else
         .ok ({s with
                   machineState.stack := e :: a :: b :: c :: d :: e :: t,
-                  machineState.gasAvailable := s.machineState.gasAvailable.natSub GasConstants.Gverylow
+                  machineState.gasAvailable := s.machineState.gasAvailable.subNat GasConstants.Gverylow
                   machineState.pc := s.machineState.pc + ⟨1⟩
                   machineState.execLength := s.machineState.execLength + 1
                   }
@@ -6361,10 +6295,7 @@ theorem step_dup5 : ∀ (s : State),
           unfold step
           simp [EVM.dup, Ethereum.State.replaceStackAndIncrPC]
           unfold Ethereum.State.incrPC
-          simp
-          apply And.intro
-          · simp [UInt256_ofNat_1]
-          · rw [Sat256.natSub_zero]
+          simp [UInt256_ofNat_1, Sat256.subNat_zero]
 
 theorem step_swap5 : ∀ (s : State),
   let I_b := s.executionEnv.code
@@ -6378,7 +6309,7 @@ theorem step_swap5 : ∀ (s : State),
         else
         .ok ({s with
                   machineState.stack := f :: b :: c :: d :: e :: a :: t,
-                  machineState.gasAvailable := s.machineState.gasAvailable.natSub GasConstants.Gverylow
+                  machineState.gasAvailable := s.machineState.gasAvailable.subNat GasConstants.Gverylow
                   machineState.pc := s.machineState.pc + ⟨1⟩
                   machineState.execLength := s.machineState.execLength + 1
                   }
@@ -6415,10 +6346,7 @@ theorem step_swap5 : ∀ (s : State),
           unfold step
           simp [EVM.swap, Ethereum.State.replaceStackAndIncrPC]
           unfold Ethereum.State.incrPC
-          simp
-          apply And.intro
-          · simp [UInt256_ofNat_1]
-          · rw [Sat256.natSub_zero]
+          simp [UInt256_ofNat_1, Sat256.subNat_zero]
 
 theorem step_dup6 : ∀ (s : State),
   let I_b := s.executionEnv.code
@@ -6432,7 +6360,7 @@ theorem step_dup6 : ∀ (s : State),
         else
         .ok ({s with
                   machineState.stack := f :: a :: b :: c :: d :: e :: f :: t,
-                  machineState.gasAvailable := s.machineState.gasAvailable.natSub GasConstants.Gverylow
+                  machineState.gasAvailable := s.machineState.gasAvailable.subNat GasConstants.Gverylow
                   machineState.pc := s.machineState.pc + ⟨1⟩
                   machineState.execLength := s.machineState.execLength + 1
                   }
@@ -6469,10 +6397,7 @@ theorem step_dup6 : ∀ (s : State),
           unfold step
           simp [EVM.dup, Ethereum.State.replaceStackAndIncrPC]
           unfold Ethereum.State.incrPC
-          simp
-          apply And.intro
-          · simp [UInt256_ofNat_1]
-          · rw [Sat256.natSub_zero]
+          simp [UInt256_ofNat_1, Sat256.subNat_zero]
 
 theorem step_swap6 : ∀ (s : State),
   let I_b := s.executionEnv.code
@@ -6486,7 +6411,7 @@ theorem step_swap6 : ∀ (s : State),
         else
         .ok ({s with
                   machineState.stack := g :: b :: c :: d :: e :: f :: a :: t,
-                  machineState.gasAvailable := s.machineState.gasAvailable.natSub GasConstants.Gverylow
+                  machineState.gasAvailable := s.machineState.gasAvailable.subNat GasConstants.Gverylow
                   machineState.pc := s.machineState.pc + ⟨1⟩
                   machineState.execLength := s.machineState.execLength + 1
                   }
@@ -6524,10 +6449,7 @@ theorem step_swap6 : ∀ (s : State),
           unfold step
           simp [EVM.swap, Ethereum.State.replaceStackAndIncrPC]
           unfold Ethereum.State.incrPC
-          simp
-          apply And.intro
-          · simp [UInt256_ofNat_1]
-          · rw [Sat256.natSub_zero]
+          simp [UInt256_ofNat_1, Sat256.subNat_zero]
 
 theorem step_dup7 : ∀ (s : State),
   let I_b := s.executionEnv.code
@@ -6541,7 +6463,7 @@ theorem step_dup7 : ∀ (s : State),
         else
         .ok ({s with
                   machineState.stack := g :: a :: b :: c :: d :: e :: f :: g :: t,
-                  machineState.gasAvailable := s.machineState.gasAvailable.natSub GasConstants.Gverylow
+                  machineState.gasAvailable := s.machineState.gasAvailable.subNat GasConstants.Gverylow
                   machineState.pc := s.machineState.pc + ⟨1⟩
                   machineState.execLength := s.machineState.execLength + 1
                   }
@@ -6579,10 +6501,7 @@ theorem step_dup7 : ∀ (s : State),
           unfold step
           simp [EVM.dup, Ethereum.State.replaceStackAndIncrPC]
           unfold Ethereum.State.incrPC
-          simp
-          apply And.intro
-          · simp [UInt256_ofNat_1]
-          · rw [Sat256.natSub_zero]
+          simp [UInt256_ofNat_1, Sat256.subNat_zero]
 
 theorem step_swap7 : ∀ (s : State),
   let I_b := s.executionEnv.code
@@ -6596,7 +6515,7 @@ theorem step_swap7 : ∀ (s : State),
         else
         .ok ({s with
                   machineState.stack := h :: b :: c :: d :: e :: f :: g :: a :: t,
-                  machineState.gasAvailable := s.machineState.gasAvailable.natSub GasConstants.Gverylow
+                  machineState.gasAvailable := s.machineState.gasAvailable.subNat GasConstants.Gverylow
                   machineState.pc := s.machineState.pc + ⟨1⟩
                   machineState.execLength := s.machineState.execLength + 1
                   }
@@ -6635,10 +6554,7 @@ theorem step_swap7 : ∀ (s : State),
           unfold step
           simp [EVM.swap, Ethereum.State.replaceStackAndIncrPC]
           unfold Ethereum.State.incrPC
-          simp
-          apply And.intro
-          · simp [UInt256_ofNat_1]
-          · rw [Sat256.natSub_zero]
+          simp [UInt256_ofNat_1, Sat256.subNat_zero]
 
 theorem step_dup8 : ∀ (s : State),
   let I_b := s.executionEnv.code
@@ -6652,7 +6568,7 @@ theorem step_dup8 : ∀ (s : State),
         else
         .ok ({s with
                   machineState.stack := h :: a :: b :: c :: d :: e :: f :: g :: h :: t,
-                  machineState.gasAvailable := s.machineState.gasAvailable.natSub GasConstants.Gverylow
+                  machineState.gasAvailable := s.machineState.gasAvailable.subNat GasConstants.Gverylow
                   machineState.pc := s.machineState.pc + ⟨1⟩
                   machineState.execLength := s.machineState.execLength + 1
                   }
@@ -6691,10 +6607,7 @@ theorem step_dup8 : ∀ (s : State),
           unfold step
           simp [EVM.dup, Ethereum.State.replaceStackAndIncrPC]
           unfold Ethereum.State.incrPC
-          simp
-          apply And.intro
-          · simp [UInt256_ofNat_1]
-          · rw [Sat256.natSub_zero]
+          simp [UInt256_ofNat_1, Sat256.subNat_zero]
 
 theorem step_swap8 : ∀ (s : State),
   let I_b := s.executionEnv.code
@@ -6708,7 +6621,7 @@ theorem step_swap8 : ∀ (s : State),
         else
         .ok ({s with
                   machineState.stack := i :: b :: c :: d :: e :: f :: g :: h :: a :: t,
-                  machineState.gasAvailable := s.machineState.gasAvailable.natSub GasConstants.Gverylow
+                  machineState.gasAvailable := s.machineState.gasAvailable.subNat GasConstants.Gverylow
                   machineState.pc := s.machineState.pc + ⟨1⟩
                   machineState.execLength := s.machineState.execLength + 1
                   }
@@ -6748,10 +6661,7 @@ theorem step_swap8 : ∀ (s : State),
           unfold step
           simp [EVM.swap, Ethereum.State.replaceStackAndIncrPC]
           unfold Ethereum.State.incrPC
-          simp
-          apply And.intro
-          · simp [UInt256_ofNat_1]
-          · rw [Sat256.natSub_zero]
+          simp [UInt256_ofNat_1, Sat256.subNat_zero]
 
 theorem step_dup9 : ∀ (s : State),
   let I_b := s.executionEnv.code
@@ -6765,7 +6675,7 @@ theorem step_dup9 : ∀ (s : State),
         else
         .ok ({s with
                   machineState.stack := i :: a :: b :: c :: d :: e :: f :: g :: h :: i :: t,
-                  machineState.gasAvailable := s.machineState.gasAvailable.natSub GasConstants.Gverylow
+                  machineState.gasAvailable := s.machineState.gasAvailable.subNat GasConstants.Gverylow
                   machineState.pc := s.machineState.pc + ⟨1⟩
                   machineState.execLength := s.machineState.execLength + 1
                   }
@@ -6805,10 +6715,7 @@ theorem step_dup9 : ∀ (s : State),
           unfold step
           simp [EVM.dup, Ethereum.State.replaceStackAndIncrPC]
           unfold Ethereum.State.incrPC
-          simp
-          apply And.intro
-          · simp [UInt256_ofNat_1]
-          · rw [Sat256.natSub_zero]
+          simp [UInt256_ofNat_1, Sat256.subNat_zero]
 
 theorem step_swap9 : ∀ (s : State),
   let I_b := s.executionEnv.code
@@ -6822,7 +6729,7 @@ theorem step_swap9 : ∀ (s : State),
         else
         .ok ({s with
                   machineState.stack := j :: b :: c :: d :: e :: f :: g :: h :: i :: a :: t,
-                  machineState.gasAvailable := s.machineState.gasAvailable.natSub GasConstants.Gverylow
+                  machineState.gasAvailable := s.machineState.gasAvailable.subNat GasConstants.Gverylow
                   machineState.pc := s.machineState.pc + ⟨1⟩
                   machineState.execLength := s.machineState.execLength + 1
                   }
@@ -6863,10 +6770,7 @@ theorem step_swap9 : ∀ (s : State),
           unfold step
           simp [EVM.swap, Ethereum.State.replaceStackAndIncrPC]
           unfold Ethereum.State.incrPC
-          simp
-          apply And.intro
-          · simp [UInt256_ofNat_1]
-          · rw [Sat256.natSub_zero]
+          simp [UInt256_ofNat_1, Sat256.subNat_zero]
 
 theorem step_dup10 : ∀ (s : State),
   let I_b := s.executionEnv.code
@@ -6880,7 +6784,7 @@ theorem step_dup10 : ∀ (s : State),
         else
         .ok ({s with
                   machineState.stack := j :: a :: b :: c :: d :: e :: f :: g :: h :: i :: j :: t,
-                  machineState.gasAvailable := s.machineState.gasAvailable.natSub GasConstants.Gverylow
+                  machineState.gasAvailable := s.machineState.gasAvailable.subNat GasConstants.Gverylow
                   machineState.pc := s.machineState.pc + ⟨1⟩
                   machineState.execLength := s.machineState.execLength + 1
                   }
@@ -6921,10 +6825,7 @@ theorem step_dup10 : ∀ (s : State),
           unfold step
           simp [EVM.dup, Ethereum.State.replaceStackAndIncrPC]
           unfold Ethereum.State.incrPC
-          simp
-          apply And.intro
-          · simp [UInt256_ofNat_1]
-          · rw [Sat256.natSub_zero]
+          simp [UInt256_ofNat_1, Sat256.subNat_zero]
 
 theorem step_swap10 : ∀ (s : State),
   let I_b := s.executionEnv.code
@@ -6938,7 +6839,7 @@ theorem step_swap10 : ∀ (s : State),
         else
         .ok ({s with
                   machineState.stack := k :: b :: c :: d :: e :: f :: g :: h :: i :: j :: a :: t,
-                  machineState.gasAvailable := s.machineState.gasAvailable.natSub GasConstants.Gverylow
+                  machineState.gasAvailable := s.machineState.gasAvailable.subNat GasConstants.Gverylow
                   machineState.pc := s.machineState.pc + ⟨1⟩
                   machineState.execLength := s.machineState.execLength + 1
                   }
@@ -6980,10 +6881,7 @@ theorem step_swap10 : ∀ (s : State),
           unfold step
           simp [EVM.swap, Ethereum.State.replaceStackAndIncrPC]
           unfold Ethereum.State.incrPC
-          simp
-          apply And.intro
-          · simp [UInt256_ofNat_1]
-          · rw [Sat256.natSub_zero]
+          simp [UInt256_ofNat_1, Sat256.subNat_zero]
 
 theorem step_dup11 : ∀ (s : State),
   let I_b := s.executionEnv.code
@@ -6997,7 +6895,7 @@ theorem step_dup11 : ∀ (s : State),
         else
         .ok ({s with
                   machineState.stack := k :: a :: b :: c :: d :: e :: f :: g :: h :: i :: j :: k :: t,
-                  machineState.gasAvailable := s.machineState.gasAvailable.natSub GasConstants.Gverylow
+                  machineState.gasAvailable := s.machineState.gasAvailable.subNat GasConstants.Gverylow
                   machineState.pc := s.machineState.pc + ⟨1⟩
                   machineState.execLength := s.machineState.execLength + 1
                   }
@@ -7039,10 +6937,7 @@ theorem step_dup11 : ∀ (s : State),
           unfold step
           simp [EVM.dup, Ethereum.State.replaceStackAndIncrPC]
           unfold Ethereum.State.incrPC
-          simp
-          apply And.intro
-          · simp [UInt256_ofNat_1]
-          · rw [Sat256.natSub_zero]
+          simp [UInt256_ofNat_1, Sat256.subNat_zero]
 
 theorem step_swap11 : ∀ (s : State),
   let I_b := s.executionEnv.code
@@ -7056,7 +6951,7 @@ theorem step_swap11 : ∀ (s : State),
         else
         .ok ({s with
                   machineState.stack := l :: b :: c :: d :: e :: f :: g :: h :: i :: j :: k :: a :: t,
-                  machineState.gasAvailable := s.machineState.gasAvailable.natSub GasConstants.Gverylow
+                  machineState.gasAvailable := s.machineState.gasAvailable.subNat GasConstants.Gverylow
                   machineState.pc := s.machineState.pc + ⟨1⟩
                   machineState.execLength := s.machineState.execLength + 1
                   }
@@ -7099,10 +6994,7 @@ theorem step_swap11 : ∀ (s : State),
           unfold step
           simp [EVM.swap, Ethereum.State.replaceStackAndIncrPC]
           unfold Ethereum.State.incrPC
-          simp
-          apply And.intro
-          · simp [UInt256_ofNat_1]
-          · rw [Sat256.natSub_zero]
+          simp [UInt256_ofNat_1, Sat256.subNat_zero]
 
 theorem step_dup12 : ∀ (s : State),
   let I_b := s.executionEnv.code
@@ -7116,7 +7008,7 @@ theorem step_dup12 : ∀ (s : State),
         else
         .ok ({s with
                   machineState.stack := l :: a :: b :: c :: d :: e :: f :: g :: h :: i :: j :: k :: l :: t,
-                  machineState.gasAvailable := s.machineState.gasAvailable.natSub GasConstants.Gverylow
+                  machineState.gasAvailable := s.machineState.gasAvailable.subNat GasConstants.Gverylow
                   machineState.pc := s.machineState.pc + ⟨1⟩
                   machineState.execLength := s.machineState.execLength + 1
                   }
@@ -7159,10 +7051,7 @@ theorem step_dup12 : ∀ (s : State),
           unfold step
           simp [EVM.dup, Ethereum.State.replaceStackAndIncrPC]
           unfold Ethereum.State.incrPC
-          simp
-          apply And.intro
-          · simp [UInt256_ofNat_1]
-          · rw [Sat256.natSub_zero]
+          simp [UInt256_ofNat_1, Sat256.subNat_zero]
 
 theorem step_swap12 : ∀ (s : State),
   let I_b := s.executionEnv.code
@@ -7176,7 +7065,7 @@ theorem step_swap12 : ∀ (s : State),
         else
         .ok ({s with
                   machineState.stack := m :: b :: c :: d :: e :: f :: g :: h :: i :: j :: k :: l :: a :: t,
-                  machineState.gasAvailable := s.machineState.gasAvailable.natSub GasConstants.Gverylow
+                  machineState.gasAvailable := s.machineState.gasAvailable.subNat GasConstants.Gverylow
                   machineState.pc := s.machineState.pc + ⟨1⟩
                   machineState.execLength := s.machineState.execLength + 1
                   }
@@ -7220,10 +7109,7 @@ theorem step_swap12 : ∀ (s : State),
           unfold step
           simp [EVM.swap, Ethereum.State.replaceStackAndIncrPC]
           unfold Ethereum.State.incrPC
-          simp
-          apply And.intro
-          · simp [UInt256_ofNat_1]
-          · rw [Sat256.natSub_zero]
+          simp [UInt256_ofNat_1, Sat256.subNat_zero]
 
 theorem step_dup13 : ∀ (s : State),
   let I_b := s.executionEnv.code
@@ -7237,7 +7123,7 @@ theorem step_dup13 : ∀ (s : State),
         else
         .ok ({s with
                   machineState.stack := m :: a :: b :: c :: d :: e :: f :: g :: h :: i :: j :: k :: l :: m :: t,
-                  machineState.gasAvailable := s.machineState.gasAvailable.natSub GasConstants.Gverylow
+                  machineState.gasAvailable := s.machineState.gasAvailable.subNat GasConstants.Gverylow
                   machineState.pc := s.machineState.pc + ⟨1⟩
                   machineState.execLength := s.machineState.execLength + 1
                   }
@@ -7281,10 +7167,7 @@ theorem step_dup13 : ∀ (s : State),
           unfold step
           simp [EVM.dup, Ethereum.State.replaceStackAndIncrPC]
           unfold Ethereum.State.incrPC
-          simp
-          apply And.intro
-          · simp [UInt256_ofNat_1]
-          · rw [Sat256.natSub_zero]
+          simp [UInt256_ofNat_1, Sat256.subNat_zero]
 
 theorem step_swap13 : ∀ (s : State),
   let I_b := s.executionEnv.code
@@ -7298,7 +7181,7 @@ theorem step_swap13 : ∀ (s : State),
         else
         .ok ({s with
                   machineState.stack := n :: b :: c :: d :: e :: f :: g :: h :: i :: j :: k :: l :: m :: a :: t,
-                  machineState.gasAvailable := s.machineState.gasAvailable.natSub GasConstants.Gverylow
+                  machineState.gasAvailable := s.machineState.gasAvailable.subNat GasConstants.Gverylow
                   machineState.pc := s.machineState.pc + ⟨1⟩
                   machineState.execLength := s.machineState.execLength + 1
                   }
@@ -7343,10 +7226,7 @@ theorem step_swap13 : ∀ (s : State),
           unfold step
           simp [EVM.swap, Ethereum.State.replaceStackAndIncrPC]
           unfold Ethereum.State.incrPC
-          simp
-          apply And.intro
-          · simp [UInt256_ofNat_1]
-          · rw [Sat256.natSub_zero]
+          simp [UInt256_ofNat_1, Sat256.subNat_zero]
 
 theorem step_dup14 : ∀ (s : State),
   let I_b := s.executionEnv.code
@@ -7360,7 +7240,7 @@ theorem step_dup14 : ∀ (s : State),
         else
         .ok ({s with
                   machineState.stack := n :: a :: b :: c :: d :: e :: f :: g :: h :: i :: j :: k :: l :: m :: n :: t,
-                  machineState.gasAvailable := s.machineState.gasAvailable.natSub GasConstants.Gverylow
+                  machineState.gasAvailable := s.machineState.gasAvailable.subNat GasConstants.Gverylow
                   machineState.pc := s.machineState.pc + ⟨1⟩
                   machineState.execLength := s.machineState.execLength + 1
                   }
@@ -7405,10 +7285,7 @@ theorem step_dup14 : ∀ (s : State),
           unfold step
           simp [EVM.dup, Ethereum.State.replaceStackAndIncrPC]
           unfold Ethereum.State.incrPC
-          simp
-          apply And.intro
-          · simp [UInt256_ofNat_1]
-          · rw [Sat256.natSub_zero]
+          simp [UInt256_ofNat_1, Sat256.subNat_zero]
 
 theorem step_swap14 : ∀ (s : State),
   let I_b := s.executionEnv.code
@@ -7422,7 +7299,7 @@ theorem step_swap14 : ∀ (s : State),
         else
         .ok ({s with
                   machineState.stack := o :: b :: c :: d :: e :: f :: g :: h :: i :: j :: k :: l :: m :: n :: a :: t,
-                  machineState.gasAvailable := s.machineState.gasAvailable.natSub GasConstants.Gverylow
+                  machineState.gasAvailable := s.machineState.gasAvailable.subNat GasConstants.Gverylow
                   machineState.pc := s.machineState.pc + ⟨1⟩
                   machineState.execLength := s.machineState.execLength + 1
                   }
@@ -7468,10 +7345,7 @@ theorem step_swap14 : ∀ (s : State),
           unfold step
           simp [EVM.swap, Ethereum.State.replaceStackAndIncrPC]
           unfold Ethereum.State.incrPC
-          simp
-          apply And.intro
-          · simp [UInt256_ofNat_1]
-          · rw [Sat256.natSub_zero]
+          simp [UInt256_ofNat_1, Sat256.subNat_zero]
 
 theorem step_dup15 : ∀ (s : State),
   let I_b := s.executionEnv.code
@@ -7485,7 +7359,7 @@ theorem step_dup15 : ∀ (s : State),
         else
         .ok ({s with
                   machineState.stack := o :: a :: b :: c :: d :: e :: f :: g :: h :: i :: j :: k :: l :: m :: n :: o :: t,
-                  machineState.gasAvailable := s.machineState.gasAvailable.natSub GasConstants.Gverylow
+                  machineState.gasAvailable := s.machineState.gasAvailable.subNat GasConstants.Gverylow
                   machineState.pc := s.machineState.pc + ⟨1⟩
                   machineState.execLength := s.machineState.execLength + 1
                   }
@@ -7531,10 +7405,7 @@ theorem step_dup15 : ∀ (s : State),
           unfold step
           simp [EVM.dup, Ethereum.State.replaceStackAndIncrPC]
           unfold Ethereum.State.incrPC
-          simp
-          apply And.intro
-          · simp [UInt256_ofNat_1]
-          · rw [Sat256.natSub_zero]
+          simp [UInt256_ofNat_1, Sat256.subNat_zero]
 
 theorem step_swap15 : ∀ (s : State),
   let I_b := s.executionEnv.code
@@ -7548,7 +7419,7 @@ theorem step_swap15 : ∀ (s : State),
         else
         .ok ({s with
                   machineState.stack := p :: b :: c :: d :: e :: f :: g :: h :: i :: j :: k :: l :: m :: n :: o :: a :: t,
-                  machineState.gasAvailable := s.machineState.gasAvailable.natSub GasConstants.Gverylow
+                  machineState.gasAvailable := s.machineState.gasAvailable.subNat GasConstants.Gverylow
                   machineState.pc := s.machineState.pc + ⟨1⟩
                   machineState.execLength := s.machineState.execLength + 1
                   }
@@ -7595,10 +7466,7 @@ theorem step_swap15 : ∀ (s : State),
           unfold step
           simp [EVM.swap, Ethereum.State.replaceStackAndIncrPC]
           unfold Ethereum.State.incrPC
-          simp
-          apply And.intro
-          · simp [UInt256_ofNat_1]
-          · rw [Sat256.natSub_zero]
+          simp [UInt256_ofNat_1, Sat256.subNat_zero]
 
 theorem step_dup16 : ∀ (s : State),
   let I_b := s.executionEnv.code
@@ -7612,7 +7480,7 @@ theorem step_dup16 : ∀ (s : State),
         else
         .ok ({s with
                   machineState.stack := p :: a :: b :: c :: d :: e :: f :: g :: h :: i :: j :: k :: l :: m :: n :: o :: p :: t,
-                  machineState.gasAvailable := s.machineState.gasAvailable.natSub GasConstants.Gverylow
+                  machineState.gasAvailable := s.machineState.gasAvailable.subNat GasConstants.Gverylow
                   machineState.pc := s.machineState.pc + ⟨1⟩
                   machineState.execLength := s.machineState.execLength + 1
                   }
@@ -7659,10 +7527,7 @@ theorem step_dup16 : ∀ (s : State),
           unfold step
           simp [EVM.dup, Ethereum.State.replaceStackAndIncrPC]
           unfold Ethereum.State.incrPC
-          simp
-          apply And.intro
-          · simp [UInt256_ofNat_1]
-          · rw [Sat256.natSub_zero]
+          simp [UInt256_ofNat_1, Sat256.subNat_zero]
 
 theorem step_swap16 : ∀ (s : State),
   let I_b := s.executionEnv.code
@@ -7676,7 +7541,7 @@ theorem step_swap16 : ∀ (s : State),
         else
         .ok ({s with
                   machineState.stack := q :: b :: c :: d :: e :: f :: g :: h :: i :: j :: k :: l :: m :: n :: o :: p :: a :: t,
-                  machineState.gasAvailable := s.machineState.gasAvailable.natSub GasConstants.Gverylow
+                  machineState.gasAvailable := s.machineState.gasAvailable.subNat GasConstants.Gverylow
                   machineState.pc := s.machineState.pc + ⟨1⟩
                   machineState.execLength := s.machineState.execLength + 1
                   }
@@ -7724,7 +7589,4 @@ theorem step_swap16 : ∀ (s : State),
           unfold step
           simp [EVM.swap, Ethereum.State.replaceStackAndIncrPC]
           unfold Ethereum.State.incrPC
-          simp
-          apply And.intro
-          · simp [UInt256_ofNat_1]
-          · rw [Sat256.natSub_zero]
+          simp [UInt256_ofNat_1, Sat256.subNat_zero]
